src/guarding/storage_protocol/protocol.v
@@ -11,145 +11,400 @@ From iris.proofmode Require Import coq_tactics.
 
 From stdpp Require Export namespaces.
 
-(*From iris.base_logic.lib Require Export wsat.*)
-
-Require Import guarding.storage_protocol.inved.
-Require Import guarding.guard.
+Require Import guarding.internal.inved.
 Require Import guarding.internal.auth_frag_util.
+Require Import guarding.internal.wsat_util.
+Require Import guarding.guard.
 Require Import guarding.factoring_props.
 Require Import guarding.own_and_own_sep.
-Require Import guarding.internal.wsat_util.
+Require Import guarding.own_and.
 
-(*
-Context {Σ: gFunctors}.
-Context `{!invGS Σ}.
-*)
+Class SPRel (P : Type) (B : Type) := sp_rel : P → B → Prop.
 
-Class Interp (P : Type) (B : Type) := interp : P → B.
+Class SPInv (P : Type) := sp_inv : P → Prop.
+Class SPInterp (P : Type) (B : Type) := sp_interp : P → B.
 
-
-Record StorageMixin P B
-    `{Equiv P, PCore P, Op P, Valid P, PInv P, Unit P}
-    {equ: @Equivalence P (≡)}
-    `{Equiv B, PCore B, Op B, Valid B, Unit B, Interp P B}
+Class StorageMixin P B
+    `{Equiv P, PCore P, Op P, Valid P, Unit P}
+    {equ_p: @Equivalence P (≡)}
+    `{Equiv B, PCore B, Op B, Valid B, Unit B, SPRel P B}
+    {equ_b: @Equivalence B (≡)}
 := {
-    protocol_mixin: ProtocolMixin P;
-    base_ra_mixin: RAMixin B; (* completely ignore core *)
+    protocol_ra_mixin: RAMixin P; (* ignore valid *)
+    base_ra_mixin: RAMixin B; (* ignore core *)
     
+    protocol_unit_left_id : LeftId equiv (ε : P) op;
     base_unit_left_id : LeftId equiv (ε : B) op;
 
-    interp_proper: Proper ((≡) ==> (≡)) interp;
-    interp_val: ∀ p: P , pinv p -> ✓ interp p;
+    sp_rel_proper: Proper ((≡) ==> (≡) ==> (↔)) sp_rel;
+    interp_val: ∀ (p: P) (b: B) , sp_rel p b → ✓ b;
 }. 
+Global Arguments protocol_ra_mixin (P B) {_ _ _ _ _ _ _ _ _ _ _ _ _} (_).
+Global Arguments base_ra_mixin (P B) {_ _ _ _ _ _ _ _ _ _ _ _ _} (_).
+Global Arguments protocol_unit_left_id (P B) {_ _ _ _ _ _ _ _ _ _ _ _ _} (_).
+Global Arguments base_unit_left_id (P B) {_ _ _ _ _ _ _ _ _ _ _ _ _} (_).
+Global Arguments sp_rel_proper (P B) {_ _ _ _ _ _ _ _ _ _ _ _ _} (_).
+Global Arguments interp_val (P B) {_ _ _ _ _ _ _ _ _ _ _ _ _} (_).
 
+Class StorageMixinII P B
+    `{Equiv P, PCore P, Op P, Valid P, Unit P}
+    {equ_p: @Equivalence P (≡)}
+    `{Equiv B, PCore B, Op B, Valid B, Unit B, SPInv P, SPInterp P B}
+    {equ_b: @Equivalence B (≡)}
+:= {
+    protocol_ra_mixin_ii: RAMixin P;
+    base_ra_mixin_ii: RAMixin B; (* completely ignore core *)
+    
+    protocol_unit_left_id_ii : LeftId equiv (ε : P) op;
+    base_unit_left_id_ii : LeftId equiv (ε : B) op;
+
+    sp_inv_proper_ii: Proper ((≡) ==> (↔)) sp_inv;
+    sp_interp_proper_ii: Proper ((≡) ==> (≡)) sp_interp;
+    interp_val_ii: ∀ (p: P) , sp_inv p → ✓ (sp_interp p);
+}.
+Global Arguments protocol_ra_mixin_ii (P B) {_ _ _ _ _ _ _ _ _ _ _ _ _ _} (_).
+Global Arguments base_ra_mixin_ii (P B) {_ _ _ _ _ _ _ _ _ _ _ _ _ _} (_).
+Global Arguments protocol_unit_left_id_ii (P B) {_ _ _ _ _ _ _ _ _ _ _ _ _ _} (_).
+Global Arguments base_unit_left_id_ii (P B) {_ _ _ _ _ _ _ _ _ _ _ _ _ _} (_).
+Global Arguments sp_inv_proper_ii (P B) {_ _ _ _ _ _ _ _ _ _ _ _ _ _} (_).
+Global Arguments sp_interp_proper_ii (P B) {_ _ _ _ _ _ _ _ _ _ _ _ _ _} (_).
+Global Arguments interp_val_ii (P B) {_ _ _ _ _ _ _ _ _ _ _ _ _ _} (_).
 
 Section PropMap.
   Context {Σ: gFunctors}.
-  
   Context `{Equiv B, Op B, Valid B, Unit B}.
   
-  Definition wf_prop_map (f: B -> iProp Σ) :=
+  Definition wf_prop_map (f: B → iProp Σ) :=
       Proper ((≡) ==> (≡)) f
-      /\ f ε ≡ (True)%I
-      /\ (∀ a b , ✓(a ⋅ b) -> f (a ⋅ b) ≡ (f a ∗ f b) % I).
-      
-  
+      ∧ f ε ≡ (True)%I
+      ∧ (∀ a b , ✓(a ⋅ b) → f (a ⋅ b) ≡ (f a ∗ f b) % I).
 End PropMap.
 
-Section StorageLogic.
+Section StorageRelations.
+  Context `{Equiv P, PCore P, Op P, Valid P, Unit P, SPRel P B}.
   Context `{Equiv B, PCore B, Op B, Valid B, Unit B}.
-  Context `{Equiv P, PCore P, Op P, PInv P, Valid P, Unit P, Interp P B}.
-  
   
   Definition storage_protocol_guards (p: P) (b: B) :=
-      ∀ q , pinv (p ⋅ q) -> b ≼ interp (p ⋅ q).
+      ∀ q (t: B) , sp_rel (p ⋅ q) t → b ≼ t.
       
   Definition storage_protocol_exchange (p1 p2: P) (b1 b2: B)  :=
-      ∀ q , pinv (p1 ⋅ q) -> pinv (p2 ⋅ q)
-          /\ ✓(interp (p1 ⋅ q) ⋅ b1)
-          /\ interp (p1 ⋅ q) ⋅ b1 ≡ interp (p2 ⋅ q) ⋅ b2.
+      ∀ q t1, sp_rel (p1 ⋅ q) t1 →
+          ∃ t2, sp_rel (p2 ⋅ q) t2
+          ∧ ✓(t1 ⋅ b1)
+          ∧ t1 ⋅ b1 ≡ t2 ⋅ b2.
           
   Definition storage_protocol_update (p1 p2: P) :=
-      ∀ q , pinv (p1 ⋅ q) -> pinv (p2 ⋅ q)
-          /\ interp (p1 ⋅ q) ≡ interp (p2 ⋅ q).
+      ∀ q t1 , sp_rel (p1 ⋅ q) t1 → sp_rel (p2 ⋅ q) t1.
           
   Definition storage_protocol_withdraw (p1 p2: P) (b2: B)  :=
-      ∀ q , pinv (p1 ⋅ q) -> pinv (p2 ⋅ q)
-          /\ interp (p1 ⋅ q) ≡ interp (p2 ⋅ q) ⋅ b2.
+      ∀ q t1 , sp_rel (p1 ⋅ q) t1 → ∃ t2, sp_rel (p2 ⋅ q) t2
+          ∧ t1 ≡ t2 ⋅ b2.
           
   Definition storage_protocol_deposit (p1 p2: P) (b1: B)  :=
-      ∀ q , pinv (p1 ⋅ q) -> pinv (p2 ⋅ q)
-          /\ ✓(interp (p1 ⋅ q) ⋅ b1)
-          /\ interp (p1 ⋅ q) ⋅ b1 ≡ interp (p2 ⋅ q).
+      ∀ q t1 , sp_rel (p1 ⋅ q) t1 → ∃ t2, sp_rel (p2 ⋅ q) t2
+          ∧ ✓(t1 ⋅ b1)
+          ∧ t1 ⋅ b1 ≡ t2.
           
-  Definition storage_protocol_exchange_nondeterministic (p1: P) (b1: B) (output_ok: P -> B -> Prop)  :=
-      ∀ q , pinv (p1 ⋅ q) -> ∃ p2 b2 , output_ok p2 b2
-          /\ pinv (p2 ⋅ q)
-          /\ ✓(interp (p1 ⋅ q) ⋅ b1)
-          /\ interp (p1 ⋅ q) ⋅ b1 ≡ interp (p2 ⋅ q) ⋅ b2.
+  Definition storage_protocol_exchange_nondeterministic (p1: P) (b1: B) (output_ok: P → B → Prop)  :=
+      ∀ q t1 , sp_rel (p1 ⋅ q) t1 → ∃ p2 b2 t2 , output_ok p2 b2
+          ∧ sp_rel (p2 ⋅ q) t2
+          ∧ ✓(t1 ⋅ b1)
+          ∧ t1 ⋅ b1 ≡ t2 ⋅ b2.
+End StorageRelations.
 
+Section StorageRelationsII.
+  Context {P B: Type}.
+  Context `{Equiv P, PCore P, Op P, Valid P, Unit P, SPInv P, SPInterp P B}.
+  Context `{Equiv B, PCore B, Op B, Valid B, Unit B}.
+  
+  Definition storage_protocol_guards_ii (p: P) (b: B) :=
+      ∀ q , sp_inv (p ⋅ q) → b ≼ sp_interp (p ⋅ q).
+      
+  Definition storage_protocol_exchange_ii (p1 p2: P) (b1 b2: B)  :=
+      ∀ q , sp_inv (p1 ⋅ q) → sp_inv (p2 ⋅ q)
+          ∧ ✓(sp_interp (p1 ⋅ q) ⋅ b1)
+          ∧ sp_interp (p1 ⋅ q) ⋅ b1 ≡ sp_interp (p2 ⋅ q) ⋅ b2.
           
-  Context {equ: Equivalence (≡@{P})}.
-  Context {equb: Equivalence (≡@{B})}.
-  Context {storage_mixin: StorageMixin P B}.
+  Definition storage_protocol_update_ii (p1 p2: P) :=
+      ∀ q , sp_inv (p1 ⋅ q) → sp_inv (p2 ⋅ q)
+          ∧ sp_interp (p1 ⋅ q) ≡ sp_interp (p2 ⋅ q).
+          
+  Definition storage_protocol_withdraw_ii (p1 p2: P) (b2: B)  :=
+      ∀ q , sp_inv (p1 ⋅ q) → sp_inv (p2 ⋅ q)
+          ∧ sp_interp (p1 ⋅ q) ≡ sp_interp (p2 ⋅ q) ⋅ b2.
+          
+  Definition storage_protocol_deposit_ii (p1 p2: P) (b1: B)  :=
+      ∀ q , sp_inv (p1 ⋅ q) → sp_inv (p2 ⋅ q)
+          ∧ ✓(sp_interp (p1 ⋅ q) ⋅ b1)
+          ∧ sp_interp (p1 ⋅ q) ⋅ b1 ≡ sp_interp (p2 ⋅ q).
+          
+  Definition storage_protocol_exchange_nondeterministic_ii (p1: P) (b1: B) (output_ok: P → B → Prop) :=
+      ∀ q , sp_inv (p1 ⋅ q) → ∃ p2 b2 , output_ok p2 b2
+          ∧ sp_inv (p2 ⋅ q)
+          ∧ ✓(sp_interp (p1 ⋅ q) ⋅ b1)
+          ∧ sp_interp (p1 ⋅ q) ⋅ b1 ≡ sp_interp (p2 ⋅ q) ⋅ b2.
+End StorageRelationsII.
 
-  Instance sm_interp_proper
-      : Proper ((≡) ==> (≡)) (interp).
-  Proof using B H H0 H1 H10 H2 H3 H4 H5 H6 H7 H8 H9 P equ storage_mixin.
+Section StorageRelationsIILemmas.
+  Context `{Equiv B, PCore B, Op B, Valid B, Unit B}.
+  Context `{Equiv P, PCore P, Op P, Valid P, Unit P, SPInv P, SPInterp P B}.
+  Context {equ_p: @Equivalence P (≡)}.
+  Context {equ_b: @Equivalence B (≡)}.
+  Context {storage_mixin_ii: StorageMixinII P B}.
+  
+  Global Instance sp_rel_of_ii : SPRel P B := λ p b , sp_inv p ∧ sp_interp p ≡ b.
+          
+  Local Instance base_ra_op_proper : Proper ((≡) ==> (≡) ==> (≡)) (@op B _).
+  Proof using storage_mixin_ii.
+    unfold Proper, "==>". intros x y Heq x0 y0 Heq0.
+    enough (x ⋅ x0 ≡ y ⋅ x0) as X.
+    { setoid_rewrite X.
+      eapply (ra_op_proper _ (base_ra_mixin_ii _ _ storage_mixin_ii)). trivial. }
+    setoid_rewrite (ra_comm _ (base_ra_mixin_ii _ _ storage_mixin_ii) x x0).
+    setoid_rewrite (ra_comm _ (base_ra_mixin_ii _ _ storage_mixin_ii) y x0).
+    eapply (ra_op_proper _ (base_ra_mixin_ii _ _ storage_mixin_ii)). trivial.
+  Qed.
+  
+  Local Instance base_ra_valid_proper : Proper ((≡) ==> (↔)) (@valid B _).
+  Proof using storage_mixin_ii.
+    unfold Proper, "==>". intros x y Heq. split.
+    - intros Hval. eapply (ra_validN_proper _ (base_ra_mixin_ii _ _ storage_mixin_ii)).
+        { eapply Heq. } apply Hval.
+    - intros Hval. eapply (ra_validN_proper _ (base_ra_mixin_ii _ _ storage_mixin_ii)).
+        { symmetry. eapply Heq. } apply Hval.
+  Qed.
+  
+  Lemma eq_storage_protocol_guards_ii (p: P) (b: B)
+    : storage_protocol_guards p b ↔ storage_protocol_guards_ii p b.
+  Proof using equ_b.
+    unfold storage_protocol_guards, storage_protocol_guards_ii. split.
+    - intros Q q spi. apply (Q q). split; trivial.
+    - intros Q q t [Hi Heq]. destruct (Q q Hi) as [z Hj]. exists z.
+      setoid_rewrite <- Heq. trivial.
+  Qed.
+   
+  Lemma eq_storage_protocol_exchange_ii (p1 p2: P) (b1 b2: B)
+    : storage_protocol_exchange p1 p2 b1 b2 ↔ storage_protocol_exchange_ii p1 p2 b1 b2.
+  Proof using storage_mixin_ii.
+    unfold storage_protocol_exchange, storage_protocol_exchange_ii. split.
+    - intros Q q Hspi. destruct (Q q (sp_interp (p1 ⋅ q))) as [b [[Hbi Hbin] [Hc1 Hceq]]].
+      + split; trivial.
+      + split; trivial. split; trivial. setoid_rewrite Hbin. trivial.
+    - intros Q q t1 [Hspi Heq]. exists (sp_interp (p2 ⋅ q)).
+      destruct (Q q Hspi) as [Hspi2 [Hval Heq2]]. split; trivial.
+      + split; trivial.
+      + split; trivial.
+        * setoid_rewrite <- Heq; trivial.
+        * setoid_rewrite <- Heq; trivial.
+  Qed.
+  
+  Lemma eq_storage_protocol_update_ii (p1 p2: P)
+    : storage_protocol_update p1 p2 ↔ storage_protocol_update_ii p1 p2.
+  Proof using equ_b.
+    unfold storage_protocol_update, storage_protocol_update_ii. split.
+    - intros Q q Hspi. destruct (Q q (sp_interp (p1 ⋅ q))) as [b Hb].
+      + split; trivial.
+      + split; trivial.
+    - intros Q q t1 [Hspi Heq].
+      destruct (Q q Hspi) as [Hspi2 Heq2]. split; trivial.
+      + setoid_rewrite <- Heq2. trivial.
+  Qed.
+  
+  Lemma eq_storage_protocol_withdraw_ii (p1 p2: P) (b2: B)
+    : storage_protocol_withdraw p1 p2 b2 ↔ storage_protocol_withdraw_ii p1 p2 b2.
+  Proof using storage_mixin_ii.
+    unfold storage_protocol_withdraw, storage_protocol_withdraw_ii. split.
+    - intros Q q Hspi. destruct (Q q (sp_interp (p1 ⋅ q))) as [b [[Hba Hbb] Hc]].
+      + split; trivial.
+      + split; trivial. setoid_rewrite Hbb. trivial.
+    - intros Q q t1 [Hspi Heq]. exists (sp_interp (p2 ⋅ q)).
+      destruct (Q q Hspi) as [Hspi2 Heq2]. split; trivial.
+      + split; trivial.
+      + setoid_rewrite <- Heq. trivial.
+  Qed.
+  
+  Lemma eq_storage_protocol_deposit_ii (p1 p2: P) (b1: B)
+    : storage_protocol_deposit p1 p2 b1 ↔ storage_protocol_deposit_ii p1 p2 b1.
+  Proof using storage_mixin_ii.
+    unfold storage_protocol_deposit, storage_protocol_deposit_ii. split.
+    - intros Q q Hspi. destruct (Q q (sp_interp (p1 ⋅ q))) as [b [[Hbi Hbin] [Hc1 Hceq]]].
+      + split; trivial.
+      + split; trivial. split; trivial. setoid_rewrite Hbin. trivial.
+    - intros Q q t1 [Hspi Heq]. exists (sp_interp (p2 ⋅ q)).
+      destruct (Q q Hspi) as [Hspi2 [Hval Heq2]]. split; trivial.
+      + split; trivial.
+      + split; trivial.
+        * setoid_rewrite <- Heq; trivial.
+        * setoid_rewrite <- Heq; trivial.
+  Qed.
+  
+  Lemma eq_storage_protocol_exchange_nondeterministic_ii (p1: P) (b1: B) (output_ok: P → B → Prop)
+    : storage_protocol_exchange_nondeterministic p1 b1 output_ok
+      ↔ storage_protocol_exchange_nondeterministic_ii p1 b1 output_ok.
+  Proof using storage_mixin_ii.
+    unfold storage_protocol_exchange_nondeterministic,
+      storage_protocol_exchange_nondeterministic_ii. split.
+     - intros Q q Hspi.
+        destruct (Q q (sp_interp (p1 ⋅ q))) as [p2 [b2 [t2 [Hoo [Hrel [Hval Heq]]]]]].
+      + split; trivial.
+      + destruct Hrel as [Ha Hb]. exists p2. exists b2. split; trivial. split; trivial.
+        split; trivial. setoid_rewrite Hb. trivial.
+     - intros Q q t1 [Hinv Hint]. destruct (Q q Hinv) as [p2 [b2 [Hoo [Hspinv [Hval Heq]]]]].
+        exists p2. exists b2. exists (sp_interp (p2 ⋅ q)). split; trivial.
+        split.
+        + split; trivial.
+        + split.
+          * setoid_rewrite <- Hint. trivial.
+          * setoid_rewrite <- Hint. trivial.
+  Qed.
+End StorageRelationsIILemmas.
+
+Global Instance storage_mixin_from_ii
+  `{Equiv B, PCore B, Op B, Valid B, Unit B}
+  `{Equiv P, PCore P, Op P, Valid P, Unit P, SPInv P, SPInterp P B}
+  {equ_p: @Equivalence P (≡)}
+  {equ_b: @Equivalence B (≡)}
+  (storage_mixin_ii: StorageMixinII P B) : StorageMixin P B.
+Proof.
+    split.
+     - apply (protocol_ra_mixin_ii P B storage_mixin_ii).
+     - apply (base_ra_mixin_ii P B storage_mixin_ii).
+     - apply (protocol_unit_left_id_ii P B storage_mixin_ii).
+     - apply (base_unit_left_id_ii P B storage_mixin_ii).
+     - intros x y Heq x0 y0 Heq0. split.
+        + intros [Hinv HeqX]. split.
+          * rewrite (sp_inv_proper_ii _ _ storage_mixin_ii). { apply Hinv. } symmetry.
+              apply Heq.
+          * setoid_rewrite Heq0 in HeqX.
+            rewrite (sp_interp_proper_ii _ _ storage_mixin_ii). { apply HeqX. }
+            symmetry. apply Heq.
+        + intros [Hinv HeqX]. split.
+          * rewrite (sp_inv_proper_ii _ _ storage_mixin_ii). { apply Hinv. }
+              apply Heq.
+          * setoid_rewrite <- Heq0 in HeqX.
+            rewrite (sp_interp_proper_ii _ _ storage_mixin_ii). { apply HeqX. }
+            apply Heq.
+     - intros p b [Ha Hb]. rewrite base_ra_valid_proper. 
+      { apply (interp_val_ii _ _ storage_mixin_ii). apply Ha. } { trivial. }
+Qed.
+
+Local Instance sp_rel_pinv {P B : Type} {ir: SPRel P B} : InternalPInv P :=
+  λ p , ∃ b , sp_rel p b.
+  
+Local Definition internal_protocol_mixin_storage_mixin
+    `{Equiv P, PCore P, Op P, Valid P, Unit P}
+    {equ_p: @Equivalence P (≡)}
+    `{Equiv B, PCore B, Op B, Valid B, Unit B, SPRel P B}
+    {equ_b: @Equivalence B (≡)}
+    (storage_mixin: StorageMixin P B)
+    : InternalProtocolMixin P.
+Proof.
+  destruct storage_mixin as [Q1 Q2 Q3 Q4 irp Q5]. split; trivial.
+  unfold Proper, "==>", impl. intros x y Heq. unfold pinv, sp_rel_pinv.
+  intros [b J]. unfold Proper, "==>", impl in irp.
+  setoid_rewrite (irp x y _ b b) in J; trivial. exists b. trivial.
+Qed.
+
+Class sp_logicG
+    `{Equiv P, PCore P, Op P, Valid P, Unit P} `{equ_p: @Equivalence P (≡)}
+    `{Equiv B, PCore B, Op B, Valid B, Unit B, SPRel P B} `{equ_b: @Equivalence B (≡)}
+    (storage_mixin: StorageMixin P B) Σ
+:= {
+  #[local] sp_authG :: inG Σ (authUR (inved_protocolUR
+                          (internal_protocol_mixin_storage_mixin storage_mixin)))
+}.
+
+Definition sp_logicΣ
+    `{Equiv P, PCore P, Op P, Valid P, Unit P} `{equ_p: @Equivalence P (≡)}
+    `{Equiv B, PCore B, Op B, Valid B, Unit B, SPRel P B} `{equ_b: @Equivalence B (≡)}
+    (storage_mixin: StorageMixin P B)
+: gFunctors := #[
+  GFunctor (authUR (inved_protocolUR
+                          (internal_protocol_mixin_storage_mixin storage_mixin)))
+].
+
+Global Instance subG_sp_logicΣ
+  `{Equiv P, PCore P, Op P, Valid P, Unit P} `{equ_p: @Equivalence P (≡)}
+  `{Equiv B, PCore B, Op B, Valid B, Unit B, SPRel P B} `{equ_b: @Equivalence B (≡)}
+  (storage_mixin: StorageMixin P B) Σ
+    : subG (sp_logicΣ storage_mixin) Σ → sp_logicG storage_mixin Σ.
+Proof.
+  solve_inG.
+Qed.
+
+Section StorageLogic.
+  Context {P B : Type}.
+  Context `{Equiv P, PCore P, Op P, Valid P, HPUnit: Unit P, SPRel P B}.
+  Context `{Equiv B, PCore B, Op B, Valid B, Unit B}.
+  Context `{equ_p: @Equivalence P (≡)}.
+  Context `{equ_b: @Equivalence B (≡)}.
+  Context `{storage_mixin: !StorageMixin P B}.
+
+  Local Instance sm_interp_proper
+      : Proper ((≡) ==> (≡) ==> (↔)) (sp_rel).
+  Proof using storage_mixin.
     destruct storage_mixin. trivial.
   Qed.
+  
+  Local Instance sm_pinv_proper
+      : Proper ((≡) ==> (↔)) (@pinv P sp_rel_pinv).
+  Proof using storage_mixin.
+    unfold Proper, "==>", pinv. intros x y Heq. split.
+    -  unfold sp_rel_pinv. intros [b Hx]. exists b. setoid_rewrite <- Heq. trivial.
+    -  unfold sp_rel_pinv. intros [b Hy]. exists b. setoid_rewrite Heq. trivial.
+  Qed.
 
-  Instance inved_proper
+  Local Instance inved_proper
       : Proper ((≡) ==> (≡)) (@Inved P).
   Proof.
     unfold Proper, "==>". intros.
     unfold "≡", inved_protocol_equiv. trivial.
   Qed.
                    
-  Global Instance my_discrete : CmraDiscrete (inved_protocolR (protocol_mixin P B storage_mixin)).
+  Global Instance my_discrete : CmraDiscrete (inved_protocolR (internal_protocol_mixin_storage_mixin storage_mixin)).
   Proof. apply discrete_cmra_discrete. Qed.
 
   Context {Σ: gFunctors}.
-  Context `{!inG Σ (authUR (inved_protocolUR (protocol_mixin P B storage_mixin)))}.
+  Context `{sp_i: !sp_logicG storage_mixin Σ}.
   Context `{!invGS Σ}.
   
-  Definition maps (γ: gname) (f: B -> iProp Σ) : iProp Σ :=
+  Definition sp_sto (γ: gname) (f: B → iProp Σ) : iProp Σ :=
       ⌜ wf_prop_map f ⌝ ∗
       own γ (◯ (Inved ε)) ∗
       ownI γ (
-        ∃ (state: P) ,
-          own γ (● (Inved state))
-          ∗ ⌜ pinv state ⌝
-          ∗ (f (interp state))
+        ∃ (state_t: P * B) ,
+          own γ (● (Inved (fst state_t)))
+          ∗ ⌜ sp_rel (fst state_t) (snd state_t) ⌝
+          ∗ (f (snd state_t))
       ). 
      
-  Definition p_own (γ: gname) (p: P) : iProp Σ := own γ (◯ (Inved p)).
+  Local Definition sp_own_def (γ: gname) (p: P) : iProp Σ := own γ (◯ (Inved p)).
+  Local Definition sp_own_aux : seal (@sp_own_def). Proof. by eexists. Qed.
+  Definition sp_own := sp_own_aux.(unseal).
+  Local Definition sp_own_eq : @sp_own = @sp_own_def := sp_own_aux.(seal_eq).
   
   Lemma pcore_inved_unit
     : (pcore (Inved (ε : P)) ≡ Some (Inved ε)).
-  Proof using B H H0 H1 H10 H2 H3 H4 H5 H6 H7 H8 H9 P equ inG0 storage_mixin Σ.
-    unfold pcore, inved_protocol_pcore. destruct (pcore ε) eqn:x.
-    { destruct storage_mixin. destruct protocol_mixin0. destruct protocol_ra_mixin.
-      have k := ra_pcore_l (ε: P) p x.
-      generalize k. rewrite ra_comm. rewrite protocol_unit_left_id.
+  Proof using equ_p storage_mixin.
+    unfold pcore, inved_protocol_pcore. destruct (pcore ε) as [p|] eqn:x.
+    {
+      have p_ra_mixin := (protocol_ra_mixin _ _ storage_mixin).
+      have k := ra_pcore_l _ p_ra_mixin (ε: P) p x.
+      generalize k. rewrite ra_comm; trivial. rewrite protocol_unit_left_id; trivial.
       intro R. setoid_rewrite R. trivial.
     }
     trivial.
   Qed.
   
-  Global Instance pers_own_frag_inved_unit γ : Persistent (own γ (◯ (Inved (ε: P)))).
-  Proof using B H H0 H1 H10 H2 H3 H4 H5 H6 H7 H8 H9 P equ equb inG0 invGS0 storage_mixin Σ.
-    apply own_core_persistent.
-    apply auth_frag_core_id.
-    unfold CoreId.
-    apply pcore_inved_unit.
+  Local Instance pers_own_frag_inved_unit γ : Persistent (own γ (◯ (Inved (ε: P)))).
+  Proof using equ_p.
+    apply own_core_persistent. apply auth_frag_core_id. unfold CoreId. apply pcore_inved_unit.
   Qed.
   
-  Global Instance pers_maps γ f : Persistent (maps γ f).
-  Proof using B H H0 H1 H10 H2 H3 H4 H5 H6 H7 H8 H9 P equ equb inG0 invGS0 storage_mixin Σ.
-  apply _. Qed.
-  
-  Lemma apply_timeless (X Y Z W V : iProp Σ) (ti: Timeless Z) (ti2: Timeless W)
+  Global Instance pers_sto γ f : Persistent (sp_sto γ f).
+  Proof using equ_p. apply _. Qed.
+   
+  Lemma apply_timeless_rhs4 (X Y Z W V : iProp Σ) (ti: Timeless Z) (ti2: Timeless W)
       : X ∧ (Y ∗ ▷ (Z ∗ W ∗ V)) -∗ ◇ (X ∧ (Y ∗ Z ∗ W ∗ ▷ (V))).
   Proof.
       iIntros "l".
@@ -161,7 +416,7 @@ Section StorageLogic.
       iModIntro. iFrame.
   Qed.
   
-  Lemma stuff1 (X Y Z W V : iProp Σ)
+  Lemma and_rhs3_entails (X Y Z W V : iProp Σ)
       : (X ∧ (Y ∗ Z ∗ W ∗ V)) ⊢ W.
   Proof.
     iIntros "x". iDestruct "x" as "[_ [_ [_ [w _]]]]". iFrame.
@@ -171,19 +426,15 @@ Section StorageLogic.
     (incll :
       @included (InvedProtocol P) (inved_protocol_equiv P) (inved_protocol_op P)
       (Inved p1) (Inved p2)) : p1 ≼ p2.
-  Proof using B H H0 H1 H2 H3 H4 H5 H6 H7 H8 H9 P equ inG0 storage_mixin Σ.
+  Proof using storage_mixin.
     unfold "≼" in incll. destruct incll as [z incll].
-    destruct z.
+    destruct z as [|p].
     - unfold "⋅", inved_protocol_op, "≡", inved_protocol_equiv in incll.
       unfold "≼". exists ε.
       setoid_rewrite (@comm P).
-      + destruct storage_mixin. destruct protocol_mixin0.
-          setoid_rewrite incll.
-          unfold LeftId in protocol_unit_left_id.
-          symmetry.
-          apply protocol_unit_left_id.
-      + destruct storage_mixin. destruct protocol_mixin0. destruct protocol_ra_mixin.
-          apply ra_comm.
+      + setoid_rewrite incll.
+        setoid_rewrite protocol_unit_left_id; trivial. apply storage_mixin.
+      + apply (ra_comm _ (protocol_ra_mixin _ _ storage_mixin)).
    - unfold "≡", inved_protocol_equiv, "⋅", inved_protocol_op in incll.
       unfold "≼". exists p. trivial.
   Qed.
@@ -204,29 +455,29 @@ Section StorageLogic.
   
   (* SP-Guard *)
   
-  Lemma logic_guard (p: P) (b: B) (γ: gname) (E: coPset) (f: B -> iProp Σ)
+  Lemma sp_guard (p: P) (b: B) (γ: gname) (E: coPset) (f: B → iProp Σ)
     (g: storage_protocol_guards p b)
     (is_in: γ ∈ E)
-    : maps γ f ⊢ (p_own γ p &&{ E }&&> ▷ f b).
-  Proof using B H H0 H1 H10 H2 H3 H4 H5 H6 H7 H8 H9 P equ equb inG0 invGS0 storage_mixin Σ.
-    unfold maps. iIntros "[%wfm [#ounit #oinv]]".
+    : sp_sto γ f ⊢ (sp_own γ p &&{ E }&&> ▷ f b).
+  Proof using equ_p.
+    unfold sp_sto. iIntros "[%wfm [#ounit #oinv]]".
     iDestruct (guards_from_inv _ _ E with "oinv") as "mg". { set_solver. }
-    assert (Inhabited P) as IP. { apply populate. apply ε. }
+    assert (Inhabited (P * B)) as IP. { apply populate. apply (ε, ε). }
     rewrite bi.later_exist.
-    iDestruct (guards_true E (p_own γ p)) as "gt".
-    iDestruct (guards_transitive _ (p_own γ p) True%I with "[gt mg]") as "gg".
+    iDestruct (guards_true E (sp_own γ p)) as "gt".
+    iDestruct (guards_transitive _ (sp_own γ p) True%I with "[gt mg]") as "gg".
       { iFrame "gt". iFrame "mg". }
-    iDestruct (lguards_exists_with_lhs P (p_own γ p) 
-      (λ state: P, (▷ (⌜ p ≼ state ⌝))%I)
-      (λ state: P, (▷ (own γ (● Inved state) ∗ ⌜pinv state⌝ ∗ f (interp state)))%I)
+    iDestruct (lguards_exists_with_lhs (P*B) (sp_own γ p) 
+      (λ (state_t: P*B), (▷ (⌜ p ≼ state_t.1 ⌝))%I)
+      (λ (state_t: P*B), (▷ (own γ (● Inved state_t.1) ∗ ⌜sp_rel state_t.1 state_t.2⌝ ∗ f state_t.2))%I)
       E 0
       with "[gg]") as "ggg".
     {
-      iIntros (x) "o". unfold p_own. iNext. iDestruct (auth_frag_conjunct_to_incl with "o") as "o"; trivial.
+      iIntros (x) "o". rewrite sp_own_eq. unfold sp_own_def. iNext. iDestruct (auth_frag_conjunct_to_incl with "o") as "o"; trivial.
     }
     { unfold guards. iFrame "gg". }
-    assert ((∃ x, ▷ (own γ (● Inved x) ∗ ⌜pinv x⌝ ∗ f (interp x)) ∗ ▷ ⌜p ≼ x⌝)
-      ⊣⊢ (▷ f b ∗ ▷(f b -∗ ∃ x, (own γ (● Inved x) ∗ ⌜pinv x⌝ ∗ f (interp x)) ∗ ⌜p ≼ x⌝)))
+    assert ((∃ x, ▷ (own γ (● Inved x.1) ∗ ⌜sp_rel x.1 x.2⌝ ∗ f x.2) ∗ ▷ ⌜p ≼ x.1⌝)
+      ⊣⊢ (▷ f b ∗ ▷(f b -∗ ∃ x, (own γ (● Inved x.1) ∗ ⌜sp_rel x.1 x.2⌝ ∗ f x.2) ∗ ⌜p ≼ x.1⌝)))
       as Equ.
     { iIntros. iSplit. { iIntros "r".
       rewrite <- bi.later_sep. iNext.
@@ -234,23 +485,20 @@ Section StorageLogic.
       unfold storage_protocol_guards in g.
       have p_incl_x_copy := p_incl_x.
       unfold "≼" in p_incl_x. destruct p_incl_x as [z p_incl_x].
-      assert (pinv (p ⋅ z)) as pinv_pz.
-          { destruct storage_mixin. destruct protocol_mixin0. setoid_rewrite <- p_incl_x. trivial. }
-      have b_le_interp := g z pinv_pz.
+      assert (sp_rel (p ⋅ z) state.2) as pinv_pz.
+          { setoid_rewrite <- p_incl_x. trivial. }
+      have b_le_interp := g z (state.2) pinv_pz.
       destruct b_le_interp as [bz b_le_interp].
       
-      assert (interp state ≡ b ⋅ bz) as ieqop.
-      { destruct storage_mixin. unfold interp. 
-          setoid_rewrite p_incl_x. trivial. }
-
       unfold wf_prop_map in wfm.
       destruct wfm as [fprop [funit fop]].
 
       assert (✓ (b ⋅ bz)) as is_val.
-      { destruct storage_mixin. destruct base_ra_mixin0.
-          setoid_rewrite <- ieqop. apply interp_val0. trivial. }
+      { destruct (base_ra_mixin _ _ storage_mixin).
+          setoid_rewrite <- b_le_interp.
+          apply (interp_val _ _ storage_mixin) with (p := p ⋅ z). trivial. }
           
-      setoid_rewrite ieqop.
+      setoid_rewrite b_le_interp.
       setoid_rewrite fop; trivial.
 
       iDestruct "t" as "[fb fbz]".
@@ -258,9 +506,11 @@ Section StorageLogic.
       iIntros "fb".
       iExists state.
       
-      setoid_rewrite ieqop.
+      setoid_rewrite b_le_interp.
       setoid_rewrite fop; trivial.
       iFrame. iSplit; iPureIntro; trivial.
+      setoid_rewrite p_incl_x. setoid_rewrite <- b_le_interp.
+      trivial.
     }
     { iIntros "[a b]". 
       iDestruct ("b" with "a") as "b".
@@ -272,13 +522,13 @@ Section StorageLogic.
     iApply guards_weaken_rhs_l. iFrame "ggg".
   Qed.
    
-  Lemma own_sep_inv_incll_helper_nondet (p1 st : P) (output_ok : P -> P -> Prop)
-    (cond : ∀ q : P, pinv (p1 ⋅ q) → ∃ p2 , output_ok p2 q /\ pinv (p2 ⋅ q))
-   : ∀ (z: InvedProtocol P) , pinv st -> ✓ (Inved st) -> Inved p1 ⋅ z ≡ Inved st →
-    ∃ p2 , output_ok p2 (match z with Inved z0 => z0 | Nah => ε end) /\ ✓ (Inved p2 ⋅ z).
-  Proof using B H H0 H1 H2 H3 H4 H5 H6 H7 H8 H9 P equ inG0 storage_mixin Σ.
+  Lemma own_sep_inv_incll_helper_nondet (p1 st : P) (t1 : B) (output_ok : P → P → Prop)
+    (cond : ∀ (q : P) , sp_rel (p1 ⋅ q) t1 → ∃ p2 t2 , output_ok p2 q ∧ sp_rel (p2 ⋅ q) t2)
+   : ∀ (z: InvedProtocol P) , sp_rel st t1 → ✓ (Inved st) → Inved p1 ⋅ z ≡ Inved st →
+    ∃ p2 , output_ok p2 (match z with Inved z0 => z0 | Nah => ε end) ∧ ✓ (Inved p2 ⋅ z).
+  Proof using storage_mixin.
   intros z inv v eq.
-    destruct z.
+    destruct z as [|p].
     - unfold "⋅", inved_protocol_op.
       unfold "⋅", inved_protocol_op in eq.
       unfold "≡", inved_protocol_equiv in eq.
@@ -288,28 +538,24 @@ Section StorageLogic.
       {
         unfold "✓", inved_protocol_valid in v. 
         destruct v as [v pi].
-        assert (p1 ⋅ (@ε _ H9) ≡ p1) as eq2.
-        { destruct storage_mixin. destruct protocol_mixin0.
-            destruct protocol_ra_mixin.
-            rewrite ra_comm.
-            apply protocol_unit_left_id.
+        assert (p1 ⋅ (@ε _ HPUnit) ≡ p1) as eq2.
+        { 
+            rewrite (ra_comm _ (protocol_ra_mixin _ _ storage_mixin)).
+            apply (protocol_unit_left_id P B storage_mixin).
         }
-        assert (pinv (p1 ⋅ (@ε _ H9))) as pi2.
+        assert (sp_rel (p1 ⋅ (@ε _ HPUnit)) t1) as pi2.
         {
-          destruct storage_mixin.
-          destruct protocol_mixin0.
-          unfold Proper, "==>", impl in inv_proper.
-          apply inv_proper with (x := p1); trivial.
-          apply inv_proper with (x := st); trivial.
+          setoid_rewrite eq2. setoid_rewrite eq. trivial.
         }
-        have c := cond (@ε _ H9) pi2.
-        destruct c as [p2 [oo c]].
+        have c := cond (@ε _ HPUnit) pi2.
+        destruct c as [p2 [b [oo c]]].
         exists p2.
         split. { apply oo. }
         exists ε.
         trivial.
+        unfold pinv, sp_rel_pinv. exists b. apply c.
       }
-      { destruct storage_mixin. trivial. }
+      { apply (internal_protocol_mixin_storage_mixin storage_mixin). }
     - unfold "⋅", inved_protocol_op in eq.
       unfold "≡", inved_protocol_equiv in eq.
       unfold "⋅", inved_protocol_op.
@@ -320,152 +566,40 @@ Section StorageLogic.
         unfold "✓", inved_protocol_valid.
         destruct v as [v pi].
         
-        assert (pinv (p1 ⋅ p)) as pinv1. {
-          destruct storage_mixin.
-          destruct protocol_mixin0.
-          unfold Proper, "==>", impl in inv_proper.
-          apply inv_proper with (x := p1 ⋅ p); trivial.
-          apply inv_proper with (x := st); trivial.
+        assert (sp_rel (p1 ⋅ p) t1) as pinv1. {
+          setoid_rewrite eq. trivial.
         }
         have c := cond p pinv1.
-        destruct c as [p2 [oo c]].
+        destruct c as [p2 [b [oo c]]].
         exists p2.
         split; trivial.
         exists ε.
         
-        destruct storage_mixin.
-        destruct protocol_mixin0.
-        unfold Proper, "==>", impl in inv_proper.
-        assert (p2 ⋅ p ⋅ (@ε _ H9) ≡ p2 ⋅ p) as eq2.
-        { destruct storage_mixin. destruct protocol_mixin0.
-            destruct protocol_ra_mixin.
-            rewrite ra_comm.
-            apply protocol_unit_left_id.
+        assert (p2 ⋅ p ⋅ (@ε _ HPUnit) ≡ p2 ⋅ p) as eq2.
+        { 
+            rewrite (ra_comm _ (protocol_ra_mixin _ _ storage_mixin)).
+            apply (protocol_unit_left_id _ _ storage_mixin).
         }
-        apply inv_proper with (x := p2 ⋅ p); trivial.
+        setoid_rewrite eq2. exists b. trivial.
       }
-      { destruct storage_mixin. trivial. }
+      { apply (internal_protocol_mixin_storage_mixin storage_mixin). }
   Qed.
   
-  (*
-  Lemma own_sep_inv_incll_helper (p1 p2 st : P)
-    (cond : ∀ q : P, pinv (p1 ⋅ q) → pinv (p2 ⋅ q))
-   : ∀ (z: InvedProtocol P) , ✓ (Inved st) -> Inved p1 ⋅ z ≡ Inved st → ✓ (Inved p2 ⋅ z).
-  Proof using B H H0 H1 H2 H3 H4 H5 H6 H7 H8 H9 P equ inG0 storage_mixin Σ.
-    intros z v eq.
-    destruct z.
-    - unfold "⋅", inved_protocol_op.
-      unfold "⋅", inved_protocol_op in eq.
-      unfold "≡", inved_protocol_equiv in eq.
-      unfold "✓", inved_protocol_valid. 
-      
-      setoid_rewrite <- eq in v.
-      {
-        unfold "✓", inved_protocol_valid in v. 
-        destruct v as [v pi].
-        have c := cond v pi.
-        exists v.
-        trivial.
-      }
-      { destruct storage_mixin. trivial. }
-    - unfold "⋅", inved_protocol_op in eq.
-      unfold "≡", inved_protocol_equiv in eq.
-      unfold "⋅", inved_protocol_op.
-      
-      setoid_rewrite <- eq in v.
-      {
-        unfold "✓", inved_protocol_valid in v.
-        unfold "✓", inved_protocol_valid.
-        destruct v as [v pi].
-        
-        assert (pinv (p1 ⋅ (p ⋅ v))) as pinv1. {
-          destruct storage_mixin.
-          destruct protocol_mixin0.
-          unfold Proper, "==>", impl in inv_proper.
-          apply inv_proper with (x := p1 ⋅ p ⋅ v); trivial.
-          destruct protocol_ra_mixin.
-          symmetry.
-          apply ra_assoc.
-        }
-        have c := cond (p ⋅ v) pinv1.
-        exists v.
-        
-        destruct storage_mixin.
-        destruct protocol_mixin0.
-        unfold Proper, "==>", impl in inv_proper.
-        apply inv_proper with (x := p2 ⋅ (p ⋅ v)); trivial.
-        destruct protocol_ra_mixin.
-        apply ra_assoc.
-      }
-      { destruct storage_mixin. trivial. }
-  Qed.
-  *)
-        
   Lemma op_nah (p1 state : P)
-    : Inved p1 ⋅ Nah ≡ Inved state -> p1 ≡ state.
+    : Inved p1 ⋅ Nah ≡ Inved state → p1 ≡ state.
   Proof. intros. trivial. Qed.
   
   Lemma op_inved_inved (p1 p2 p : P)
-    : Inved p1 ⋅ Inved p2 ≡ Inved p -> p1 ⋅ p2 ≡ p.
+    : Inved p1 ⋅ Inved p2 ≡ Inved p → p1 ⋅ p2 ≡ p.
   Proof. intros. trivial. Qed.
         
-  (*
-  Lemma own_sep_inv_incll γ (p1 p2 state : P)
-      (cond: ∀ q , pinv (p1 ⋅ q) -> pinv (p2 ⋅ q))
+  Lemma own_sep_inv_incll_nondet γ (p1 state : P) (t1: B) (output_ok: P → P → Prop)
+      (cond: ∀ q , sp_rel (p1 ⋅ q) t1 → ∃ p2 t2 , output_ok p2 q ∧ sp_rel (p2 ⋅ q) t2)
+      (pi: sp_rel state t1)
     : own γ (◯ Inved p1) ∗ own γ (● Inved state) ==∗
-      ∃ (z: P) , ⌜ state ≡ p1 ⋅ z ⌝ ∗ own γ (◯ Inved p2) ∗ own γ (● Inved (p2 ⋅ z)).
-  Proof.
-    iIntros "[x y]".
-    iDestruct (own_valid with "y") as "%val".
-    iMod (own_sep_auth_incll γ (Inved p1) (Inved p2) (Inved state) with "[x y]") as "x".
-    {
-      intro.
-      apply own_sep_inv_incll_helper; trivial.
-      generalize val. rewrite auth_auth_valid. trivial.
-    }
-    { iFrame. }
-    iDestruct "x" as (z) "[%eq [frag auth]]".
-    destruct z.
-    {
-      have eq0 := op_nah _ _ eq.
-      assert (Inved p2 ⋅ Nah ≡ Inved p2) as eq1 by trivial.
-      setoid_rewrite eq1.
-      iExists (ε:P).
-      assert (p2 ⋅ ε ≡ p2) as eq2.
-      { destruct storage_mixin. destruct protocol_mixin0.
-          destruct protocol_ra_mixin.
-          rewrite ra_comm.
-          apply protocol_unit_left_id.
-      }
-      setoid_rewrite eq2.
-      iFrame.
-      iPureIntro.
-      assert (p1 ⋅ ε ≡ p1) as eq3.
-      { destruct storage_mixin. destruct protocol_mixin0.
-          destruct protocol_ra_mixin.
-          rewrite ra_comm.
-          apply protocol_unit_left_id.
-      }
-      setoid_rewrite eq3. symmetry. trivial.
-    }
-    {
-      iExists p.
-      
-      assert (Inved p2 ⋅ Inved p ≡ Inved (p2 ⋅ p)) as eq0 by trivial.
-      setoid_rewrite eq0.
-      iFrame.
-      iPureIntro. symmetry. apply op_inved_inved. trivial.
-    }
-   Qed.
-   *)
-   
-   Lemma own_sep_inv_incll_nondet γ (p1 state : P) (output_ok: P -> P -> Prop)
-      (cond: ∀ q , pinv (p1 ⋅ q) -> ∃ p2 , output_ok p2 q /\ pinv (p2 ⋅ q))
-      (pi: pinv state)
-    : own γ (◯ Inved p1) ∗ own γ (● Inved state) ==∗
-      ∃ (z p2: P) , ⌜ output_ok p2 z /\ state ≡ p1 ⋅ z ⌝
+      ∃ (z p2: P) , ⌜ output_ok p2 z ∧ state ≡ p1 ⋅ z ⌝
           ∗ own γ (◯ Inved p2) ∗ own γ (● Inved (p2 ⋅ z)).
-   Proof.
+  Proof using storage_mixin.
    iIntros "[x y]".
    iDestruct (own_valid with "y") as "%val".
     iMod (own_sep_auth_incll_nondet γ (Inved p1) (Inved state)
@@ -475,27 +609,25 @@ Section StorageLogic.
     end)
      with "[x y]") as "x".
     {
-      intro. intro equi.
+      intro z. intro equi.
       assert (✓ Inved state) as val2. { generalize val. rewrite auth_auth_valid. trivial. }
-      have rr := own_sep_inv_incll_helper_nondet p1 state output_ok cond z pi val2 equi.
+      have rr := own_sep_inv_incll_helper_nondet p1 state t1 output_ok cond z pi val2 equi.
       destruct rr as [p2 [rr v]]. exists (Inved p2). split; trivial.
     }
     { iFrame. }
     iDestruct "x" as (z p2) "[%eq [frag auth]]".
     destruct eq as [big_oo eq].
-    destruct p2. { intuition. }
-    rename p into p2.
-    destruct z.
+    destruct p2 as [|p2]. { intuition. }
+    destruct z as [|p].
     {
       have eq0 := op_nah _ _ eq.
       assert (Inved p2 ⋅ Nah ≡ Inved p2) as eq1 by trivial.
       setoid_rewrite eq1.
       iExists (ε:P).
       assert (p2 ⋅ ε ≡ p2) as eq2.
-      { destruct storage_mixin. destruct protocol_mixin0.
-          destruct protocol_ra_mixin.
-          rewrite ra_comm.
-          apply protocol_unit_left_id.
+      { 
+        rewrite (ra_comm _ (protocol_ra_mixin _ _ storage_mixin)).
+        apply (protocol_unit_left_id _ _ storage_mixin).
       }
       iModIntro. iExists p2.
       setoid_rewrite eq2.
@@ -503,10 +635,9 @@ Section StorageLogic.
       iPureIntro.
       split. { trivial. }
       assert (p1 ⋅ ε ≡ p1) as eq3.
-      { destruct storage_mixin. destruct protocol_mixin0.
-          destruct protocol_ra_mixin.
-          rewrite ra_comm.
-          apply protocol_unit_left_id.
+      { 
+        rewrite (ra_comm _ (protocol_ra_mixin _ _ storage_mixin)).
+        apply (protocol_unit_left_id _ _ storage_mixin).
       }
       setoid_rewrite eq3. symmetry. trivial.
     }
@@ -518,16 +649,16 @@ Section StorageLogic.
       iModIntro. iExists p2. iFrame.
       iPureIntro. split. { apply big_oo. } symmetry. apply op_inved_inved. trivial.
     }
-   Qed.
+  Qed.
    
   Lemma own_inved_op_both (a b: P) γ :
       own γ (◯ Inved a) ∗ own γ (◯ Inved b) ⊣⊢ own γ (◯ Inved (a ⋅ b)).
   Proof.
     rewrite <- own_op.
     replace (◯ Inved a ⋅ ◯ Inved b) with (@auth_frag
-          (@inved_protocolUR P H4 H5 H6 H7 H8 H9 equ
-             (@protocol_mixin P B H4 H5 H6 H8 H7 H9 equ H H0 H1 H2 H3 H10 storage_mixin))
-          (@Inved P (@op P H6 a b))); trivial.
+          (inved_protocolUR
+                          (internal_protocol_mixin_storage_mixin storage_mixin))
+          (@Inved P (a ⋅ b))); trivial.
   Qed.
           
   Lemma own_inved_op (a b: P) γ :
@@ -538,125 +669,47 @@ Section StorageLogic.
       own γ (◯ Inved (a ⋅ b)) ⊢ own γ (◯ Inved a) ∗ own γ (◯ Inved b).
   Proof. rewrite own_inved_op_both. trivial. Qed.
     
-  (*
-  Lemma logic_exchange
-    (p1 p2: P) (b1 b2: B) (γ: gname) (f: B -> iProp Σ)
-    (exchng: storage_protocol_exchange p1 p2 b1 b2)
-    : maps γ f ⊢
-        p_own γ p1 ∗ ▷ f b1 ={ {[ γ ]} }=∗ p_own γ p2 ∗ ▷ f b2.
-  Proof using B H H0 H1 H2 H3 H4 H5 H6 H7 H8 H9 P equ equb inG0 invGS0 storage_mixin Σ.
-    unfold maps.
-    iIntros "[%wfm [#ounit #m]] [p f]".
-    rewrite fancy_updates.uPred_fupd_unseal. unfold fancy_updates.uPred_fupd_def.
-    iIntros "[w oe]".
-    iDestruct (ownI_open with "[w m oe]") as "[w [latp od]]".
-    { iFrame "w". iFrame "m". iFrame "oe". }
-    iMod (bi.later_exist_except_0 with "latp") as (state) "lat".
-    iDestruct "lat" as "[ois [ps fi]]".
-    iMod "ois" as "ois".
-    iMod "ps" as "%ps".
-    unfold p_own.
-    iMod (own_sep_inv_incll γ p1 p2 state with "[p ois]") as (z) "[%incll [p ois]]".
-    { unfold storage_protocol_exchange in exchng. intros q pi.
-        have exch := exchng q pi. intuition. }
-    { iFrame. }
-    
-    destruct wfm as [f_prop [f_unit f_op]]. (* need f Proper for the next step *)
-    
-    assert (f (interp state)
-          ≡ f(interp (p1 ⋅ z))) as equiv_interp_state.
-    {
-        setoid_rewrite incll. trivial.
-    }
-    
-    setoid_rewrite equiv_interp_state.
-    iDestruct (bi.later_sep with "[fi f]") as "f_op". { iFrame "fi". iFrame "f". }
-    
-    unfold storage_protocol_exchange in exchng.
-    assert (pinv (p1 ⋅ z)) as pinv_p1_z. {
-        destruct storage_mixin. destruct protocol_mixin0.
-        setoid_rewrite <- incll. trivial.
-    }
-
-    have exch := exchng z pinv_p1_z.
-    destruct exch as [pinv_p2_z [val_interp1 interp_eq]].
-    assert (✓ (interp (p2 ⋅ z) ⋅ b2)) as val_interp2.
-    {
-      destruct storage_mixin. destruct base_ra_mixin0.
-      setoid_rewrite <- interp_eq. trivial.
-    }
-    
-    setoid_rewrite <- f_op; trivial.
-
-    setoid_rewrite interp_eq.
-    setoid_rewrite f_op; trivial.
-    
-    iDestruct "f_op" as "[fi fb]".
-
-    iAssert ((▷ ∃ state0 : P,
-          own γ (● Inved state0) ∗ ⌜pinv state0⌝ ∗ f (interp state0))%I)
-          with "[ois fi]"
-          as "inv_to_return".
-    {
-      iModIntro. (* strip later *)
-      iExists (p2 ⋅ z). iFrame "ois". iFrame "fi".
-      iPureIntro. trivial.
-    }
-    iDestruct (ownI_close γ _ with "[w m inv_to_return od]") as "[w en]".
-    { iFrame "m". iFrame "inv_to_return". iFrame "w". iFrame "od". }
-    iModIntro. iModIntro. iFrame.
-  Qed.
-  *)
-   
-  Lemma logic_exchange_nondeterministic
-    (p1: P) (b1: B) (output_ok: P -> B -> Prop) (γ: gname) (f: B -> iProp Σ)
+  Lemma sp_exchange_nondeterministic
+    (p1: P) (b1: B) (output_ok: P → B → Prop) (γ: gname) (f: B → iProp Σ)
     (exchng: storage_protocol_exchange_nondeterministic p1 b1 output_ok)
-    : maps γ f ⊢
-        p_own γ p1 ∗ ▷ f b1 ={ {[ γ ]} }=∗
-          ∃ p2 b2 , ⌜ output_ok p2 b2 ⌝ ∗ p_own γ p2 ∗ ▷ f b2.
-  Proof using B H H0 H1 H2 H3 H4 H5 H6 H7 H8 H9 P equ equb inG0 invGS0 storage_mixin Σ.
-    unfold maps.
+    : sp_sto γ f ⊢
+        sp_own γ p1 ∗ ▷ f b1 ={ {[ γ ]} }=∗
+          ∃ p2 b2 , ⌜ output_ok p2 b2 ⌝ ∗ sp_own γ p2 ∗ ▷ f b2.
+  Proof.
+    unfold sp_sto. rewrite sp_own_eq. unfold sp_own_def.
     iIntros "[%wfm [#ounit #m]] [p f]".
     rewrite fancy_updates.uPred_fupd_unseal. unfold fancy_updates.uPred_fupd_def.
     iIntros "[w oe]".
     iDestruct (ownI_open with "[w m oe]") as "[w [latp od]]".
     { iFrame "w". iFrame "m". iFrame "oe". }
-    iMod (bi.later_exist_except_0 with "latp") as (state) "lat".
+    iMod (bi.later_exist_except_0 with "latp") as (state_t) "lat".
     iDestruct "lat" as "[ois [ps fi]]".
     iMod "ois" as "ois".
     iMod "ps" as "%ps".
-    unfold p_own.
-    iMod (own_sep_inv_incll_nondet γ p1 state (λ p2 q , ∃ b2 , output_ok p2 b2
-          /\ pinv (p2 ⋅ q)
-          /\ ✓(interp (p1 ⋅ q) ⋅ b1)
-          /\ interp (p1 ⋅ q) ⋅ b1 ≡ interp (p2 ⋅ q) ⋅ b2) with "[p ois]")
+    unfold sp_own.
+    iMod (own_sep_inv_incll_nondet γ p1 state_t.1 state_t.2 (λ p2 q , ∃ b2 t2 , output_ok p2 b2
+          ∧ sp_rel (p2 ⋅ q) t2
+          ∧ ✓(state_t.2 ⋅ b1)
+          ∧ state_t.2 ⋅ b1 ≡ t2 ⋅ b2) with "[p ois]")
         as (z p2) "[[%big_output_ok %incll] [p ois]]".
     { unfold storage_protocol_exchange in exchng. intros q pi.
-        have exch := exchng q pi. destruct exch as [p2 [b2 exch]]. exists p2. intuition. exists b2. intuition. }
+        have exch := exchng q state_t.2 pi. destruct exch as [p2 [b2 [t2 exch]]]. exists p2. exists t2. intuition. exists b2. exists t2. intuition. }
     { trivial. }
     { iFrame. }
-    destruct big_output_ok as [b2 [oo [pix [vix interp_eq]]]].
+    destruct big_output_ok as [b2 [t2 [oo [pix [vix interp_eq]]]]].
     
     destruct wfm as [f_prop [f_unit f_op]]. (* need f Proper for the next step *)
     
-    assert (f (interp state)
-          ≡ f(interp (p1 ⋅ z))) as equiv_interp_state.
-    {
-        setoid_rewrite incll. trivial.
-    }
-    
-    setoid_rewrite equiv_interp_state.
     iDestruct (bi.later_sep with "[fi f]") as "f_op". { iFrame "fi". iFrame "f". }
     
     unfold storage_protocol_exchange in exchng.
     assert (pinv (p1 ⋅ z)) as pinv_p1_z. {
-        destruct storage_mixin. destruct protocol_mixin0.
-        setoid_rewrite <- incll. trivial.
+        exists (state_t.2). setoid_rewrite <- incll. trivial.
     }
 
-    assert (✓ (interp (p2 ⋅ z) ⋅ b2)) as val_interp2.
+    assert (✓ (t2 ⋅ b2)) as val_interp2.
     {
-      destruct storage_mixin. destruct base_ra_mixin0.
+      destruct (base_ra_mixin _ _ storage_mixin).
       setoid_rewrite <- interp_eq. trivial.
     }
     
@@ -667,13 +720,13 @@ Section StorageLogic.
     
     iDestruct "f_op" as "[fi fb]".
 
-    iAssert ((▷ ∃ state0 : P,
-          own γ (● Inved state0) ∗ ⌜pinv state0⌝ ∗ f (interp state0))%I)
+    iAssert ((▷ ∃ (state0_t0 : P * B),
+          own γ (● Inved state0_t0.1) ∗ ⌜sp_rel state0_t0.1 state0_t0.2⌝ ∗ f state0_t0.2)%I)
           with "[ois fi]"
           as "inv_to_return".
     {
       iModIntro. (* strip later *)
-      iExists (p2 ⋅ z). iFrame "ois". iFrame "fi".
+      iExists (p2 ⋅ z, t2). iFrame "ois". iFrame "fi".
       iPureIntro. trivial.
     }
     iDestruct (ownI_close γ _ with "[w m inv_to_return od]") as "[w en]".
@@ -684,410 +737,32 @@ Section StorageLogic.
    
   (* SP-Exchange *)
    
-  Lemma logic_exchange
-    (p1 p2: P) (b1 b2: B) (γ: gname) (f: B -> iProp Σ)
+  Lemma sp_exchange
+    (p1 p2: P) (b1 b2: B) (γ: gname) (f: B → iProp Σ)
     (exchng: storage_protocol_exchange p1 p2 b1 b2)
-    : maps γ f ⊢
-        p_own γ p1 ∗ ▷ f b1 ={ {[ γ ]} }=∗ p_own γ p2 ∗ ▷ f b2.
-  Proof using B H H0 H1 H2 H3 H4 H5 H6 H7 H8 H9 P equ equb inG0 invGS0 storage_mixin Σ.
+    : sp_sto γ f ⊢
+        sp_own γ p1 ∗ ▷ f b1 ={ {[ γ ]} }=∗ sp_own γ p2 ∗ ▷ f b2.
+  Proof.
     iIntros "x y".
-    iDestruct (logic_exchange_nondeterministic p1 b1 (λ p b, p = p2 ∧ b = b2) γ f with "x y") as "J".
+    iDestruct (sp_exchange_nondeterministic p1 b1 (λ p b, p = p2 ∧ b = b2) γ f with "x y") as "J".
     { unfold storage_protocol_exchange in exchng.
       unfold storage_protocol_exchange_nondeterministic.
-      intros q pi. exists p2. exists b2.
-      have ex := exchng q pi. intuition.
+      intros q t1 pi. exists p2. exists b2.
+      have ex := exchng q t1 pi. destruct ex as [t2 ex]. exists t2. intuition.
     }
     iMod "J" as (p0 b0) "[[%eq1 %eq2] t]". iModIntro. rewrite eq1. rewrite eq2. iFrame.
   Qed.
    
-   (*
-  Lemma logic_exchange_with_extra_guard
-    (p1 p2 q: P) (b1 b2: B) (γ: gname) (f: B -> iProp Σ) (G: iProp Σ)
-    (exchng: storage_protocol_exchange (p1 ⋅ q) (p2 ⋅ q) b1 b2)
-    : maps γ f ∗ □ (G &&{ {[ γ ]} }&&$> p_own γ q) ⊢
-        G ∗ p_own γ p1 ∗ ▷ f b1 ={ {[ γ ]} }=∗ G ∗ p_own γ p2 ∗ ▷ f b2.
-  Proof using B H H0 H1 H2 H3 H4 H5 H6 H7 H8 H9 P equ equb inG0 invGS0 storage_mixin Σ.
-    unfold maps.
-    iIntros "[[%wfm [#ounit #m]] [#gu #kbi]] [g [p f]]".
-    rewrite fancy_updates.uPred_fupd_unseal. unfold fancy_updates.uPred_fupd_def.
-    iIntros "[w oe]".
-    iDestruct (ownI_open with "[w m oe]") as "[w [latp od]]".
-    { iFrame "w". iFrame "m". iFrame "oe". }
-    iMod (bi.later_exist_except_0 with "latp") as (state) "lat".
-    unfold fguards, guards_with.
-    iDestruct ("gu" $! G) as "gu2".
-    
-    iDestruct ("gu2" with "[g lat]") as "gu3".
-    { iFrame "g". iIntros "g". iFrame "g".
-        setoid_rewrite storage_bulk_inv_singleton. unfold storage_inv.
-        iExists ((∃ state0 : P, own γ (● Inved state0) ∗ ⌜pinv state0⌝ ∗ f (interp state0))%I).
-        iFrame "m".
-        setoid_rewrite know_bulk_inv_singleton. unfold know_inv.
-        iModIntro. iExists state. iFrame "lat".
-    }
-    
-    iMod "gu3" as "[po b]".
-    
-     iAssert ((own γ (◯ Inved q) ∧
-          (◇ ∃ state : P, G ∗ ▷
-                (own γ (● Inved state) ∗ ⌜pinv state⌝ ∗ f (interp state))))%I)
-          with "[po b]" as "x".
-      { iSplit. { iFrame. } 
-        iDestruct ("b" with "po") as "[ex t]".
-        setoid_rewrite storage_bulk_inv_singleton. unfold storage_inv.
-        iDestruct "ex" as (P0) "[#own lat]".
-        iDestruct (ownIagree γ P0 _ with "[m own]") as "eq".
-        { iSplitL. { iFrame "own". } iFrame "m". }
-        iRewrite "eq" in "lat".
-        iMod (bi.later_exist_except_0 with "lat") as (state0) "lat".
-        iExists state0. iFrame.
-      }
-      iMod (and_except0_r with "x") as "x".
-      rewrite bi.and_exist_l.
-      iDestruct "x" as (state0) "x".
-      iMod (apply_timeless with "x") as "x".
-      iDestruct (stuff1 with "x") as "%pinvs".
-      unfold p_own.
-      (*iDestruct (stuff3 γ p1 q state0 with "[p x]") as "%incll". { iFrame. }*)
-      
-      iAssert (own γ (◯ Inved q) ∧ own γ (● Inved state0) ∗ (G ∗ ⌜pinv state0⌝ ∗ ▷ f (interp state0)))%I with "[x]" as "x".
-      { iSplit. { iDestruct "x" as "[x _]". iFrame. }
-          iDestruct "x" as "[_ [x [y z]]]". iFrame. }
-      iDestruct (andsep_to_sepand_ucmra with "x") as "[x y]".
-      { apply auth_frag_disjointness. }
-      iDestruct (own_separates_out γ (◯ Inved q) (own γ (◯ Inved q) ∧ G ∗ ⌜pinv state0⌝ ∗ ▷ f (interp state0)) with "[y]") as "[y z]".
-      { iFrame "y". iIntros "[k _]". iFrame. }
-      
-      iDestruct (own_inved_op p1 q γ with "[p y]") as "own_p_q". { iFrame. }
-      iMod (own_sep_inv_incll γ (p1 ⋅ q) (p2 ⋅ q) state0 with "[own_p_q x]")
-          as (z) "[%incll [own_p_q x]]".
-      { unfold storage_protocol_exchange in exchng.
-        intro q0. have exq := exchng q0. intuition. }
-      { iFrame. }
-      
-      iDestruct (own_inved_op_split with "own_p_q") as "[p q]".
-      iDestruct ("z" with "q") as "[_ z]".
-       
-    destruct wfm as [f_prop [f_unit f_op]]. (* need f Proper for the next step *)
-    
-    assert (f (interp state0)
-          ≡ f(interp (p1 ⋅ q ⋅ z))) as equiv_interp_state.
-    {
-        setoid_rewrite incll. trivial.
-    }
-    
-    iDestruct "z" as "[g [_ fi]]".
-    setoid_rewrite equiv_interp_state.
-    iDestruct (bi.later_sep with "[fi f]") as "f_op". { iFrame "fi". iFrame "f". }
-    
-    unfold storage_protocol_exchange in exchng.
-    assert (pinv (p1 ⋅ q ⋅ z)) as pinv_p1_z. {
-        destruct storage_mixin. destruct protocol_mixin0.
-        setoid_rewrite <- incll. trivial.
-    }
-
-    have exch := exchng z pinv_p1_z.
-    destruct exch as [pinv_p2_z [val_interp1 interp_eq]].
-    assert (✓ (interp (p2 ⋅ q ⋅ z) ⋅ b2)) as val_interp2.
-    {
-      destruct storage_mixin. destruct base_ra_mixin0.
-      setoid_rewrite <- interp_eq. trivial.
-    }
-    
-    setoid_rewrite <- f_op; trivial.
-
-    setoid_rewrite interp_eq.
-    setoid_rewrite f_op; trivial.
-    
-    iDestruct "f_op" as "[fi fb]".
-
-    iAssert ((▷ ∃ state0 : P,
-          own γ (● Inved state0) ∗ ⌜pinv state0⌝ ∗ f (interp state0))%I)
-          with "[x fi]"
-          as "inv_to_return".
-    {
-      iModIntro. (* strip later *)
-      iExists (p2 ⋅ q ⋅ z). iFrame "x". iFrame "fi".
-      iPureIntro. trivial.
-    }
-    iDestruct (ownI_close γ _ with "[w m inv_to_return od]") as "[w en]".
-    { iFrame "m". iFrame "inv_to_return". iFrame "w". iFrame "od". }
-    iModIntro. iModIntro. iFrame.
-  Qed.
-  *)
-  
-  (*
-  Lemma logic_exchange_with_extra_guard_nondeterministic
-    (p1 q: P) (b1: B) (output_ok: P -> B -> Prop) (γ: gname) (f: B -> iProp Σ) (G: iProp Σ)
+  Lemma sp_exchange_with_extra_guard_nondeterministic_with_later
+    (p1 q: P) (b1: B) (output_ok: P → B → Prop) (γ: gname) (f: B → iProp Σ) (G: iProp Σ) E n
     (exchng: storage_protocol_exchange_nondeterministic (p1 ⋅ q) b1
-        (λ p2_q b2 , ∃ p2 , p2_q = p2 ⋅ q /\ output_ok p2 b2))
-    : maps γ f ∗ □ (G &&{ {[ γ ]} }&&$> p_own γ q) ⊢
-        G ∗ p_own γ p1 ∗ ▷ f b1 ={ {[ γ ]} }=∗ ∃ p2 b2 ,
-            ⌜ output_ok p2 b2 ⌝ ∗ G ∗ p_own γ p2 ∗ ▷ f b2.
-  Proof using B H H0 H1 H2 H3 H4 H5 H6 H7 H8 H9 P equ equb inG0 invGS0 storage_mixin Σ.
-    unfold maps.
-    iIntros "[[%wfm [#ounit #m]] [#gu #kbi]] [g [p f]]".
-    rewrite fancy_updates.uPred_fupd_unseal. unfold fancy_updates.uPred_fupd_def.
-    iIntros "[w oe]".
-    iDestruct (ownI_open with "[w m oe]") as "[w [latp od]]".
-    { iFrame "w". iFrame "m". iFrame "oe". }
-    iMod (bi.later_exist_except_0 with "latp") as (state) "lat".
-    unfold fguards, guards_with.
-    iDestruct ("gu" $! G) as "gu2".
-    
-    iDestruct ("gu2" with "[g lat]") as "gu3".
-    { iFrame "g". iIntros "g". iFrame "g".
-        setoid_rewrite storage_bulk_inv_singleton. unfold storage_inv.
-        iExists ((∃ state0 : P, own γ (● Inved state0) ∗ ⌜pinv state0⌝ ∗ f (interp state0))%I).
-        iFrame "m".
-        setoid_rewrite know_bulk_inv_singleton. unfold know_inv.
-        iModIntro. iExists state. iFrame "lat".
-    }
-    
-    iMod "gu3" as "[po b]".
-    
-     iAssert ((own γ (◯ Inved q) ∧
-          (◇ ∃ state : P, G ∗ ▷
-                (own γ (● Inved state) ∗ ⌜pinv state⌝ ∗ f (interp state))))%I)
-          with "[po b]" as "x".
-      { iSplit. { iFrame. } 
-        iDestruct ("b" with "po") as "[ex t]".
-        setoid_rewrite storage_bulk_inv_singleton. unfold storage_inv.
-        iDestruct "ex" as (P0) "[#own lat]".
-        iDestruct (ownIagree γ P0 _ with "[m own]") as "eq".
-        { iSplitL. { iFrame "own". } iFrame "m". }
-        iRewrite "eq" in "lat".
-        iMod (bi.later_exist_except_0 with "lat") as (state0) "lat".
-        iExists state0. iFrame.
-      }
-      iMod (and_except0_r with "x") as "x".
-      rewrite bi.and_exist_l.
-      iDestruct "x" as (state0) "x".
-      iMod (apply_timeless with "x") as "x".
-      iDestruct (stuff1 with "x") as "%pinvs".
-      unfold p_own.
-      (*iDestruct (stuff3 γ p1 q state0 with "[p x]") as "%incll". { iFrame. }*)
-      
-      iAssert (own γ (◯ Inved q) ∧ own γ (● Inved state0) ∗ (G ∗ ⌜pinv state0⌝ ∗ ▷ f (interp state0)))%I with "[x]" as "x".
-      { iSplit. { iDestruct "x" as "[x _]". iFrame. }
-          iDestruct "x" as "[_ [x [y z]]]". iFrame. }
-      iDestruct (andsep_to_sepand_ucmra with "x") as "[x y]".
-      { apply auth_frag_disjointness. }
-      iDestruct (own_separates_out γ (◯ Inved q) (own γ (◯ Inved q) ∧ G ∗ ⌜pinv state0⌝ ∗ ▷ f (interp state0)) with "[y]") as "[y z]".
-      { iFrame "y". iIntros "[k _]". iFrame. }
-      
-      iDestruct (own_inved_op p1 q γ with "[p y]") as "own_p_q". { iFrame. }
-      iMod (own_sep_inv_incll_nondet γ (p1 ⋅ q) state0 (λ p2_q r , ∃ p2 b2 , p2_q = p2 ⋅ q /\ output_ok p2 b2
-          /\ pinv ((p2 ⋅ q) ⋅ r)
-          /\ ✓(interp ((p1 ⋅ q) ⋅ r) ⋅ b1)
-          /\ interp ((p1 ⋅ q) ⋅ r) ⋅ b1 ≡ interp ((p2 ⋅ q) ⋅ r) ⋅ b2) with "[own_p_q x]")
-          as (z p2_q) "[%incll [own_p_q x]]".
-      { unfold storage_protocol_exchange_nondeterministic in exchng.
-        intro r. intro j0. have exq := exchng r j0.
-        destruct exq as [p2_q [b2 exq]].
-        destruct exq as [[p2 [eq oo]] [a b]].
-        exists (p2 ⋅ q). split.
-        { exists p2. exists b2. intuition. { rewrite <- eq. apply a. }
-            rewrite <- eq. trivial. }
-        { rewrite <- eq. apply a. }
-      }
-      { apply pinvs. }
-      { iFrame. }
-      
-      destruct incll as [[p2 [b2 [p2_q_eq bigconj]]] incll].
-      rewrite p2_q_eq.
-      iDestruct (own_inved_op_split with "own_p_q") as "[p q]".
-      iDestruct ("z" with "q") as "[_ z]".
-      
-      destruct bigconj as [oo [pix [iix interp_eq]]].
-       
-    destruct wfm as [f_prop [f_unit f_op]]. (* need f Proper for the next step *)
-    
-    assert (f (interp state0)
-          ≡ f(interp (p1 ⋅ q ⋅ z))) as equiv_interp_state.
-    {
-        setoid_rewrite incll. trivial.
-    }
-    
-    iDestruct "z" as "[g [_ fi]]".
-    setoid_rewrite equiv_interp_state.
-    iDestruct (bi.later_sep with "[fi f]") as "f_op". { iFrame "fi". iFrame "f". }
-    
-    unfold storage_protocol_exchange in exchng.
-    assert (pinv (p1 ⋅ q ⋅ z)) as pinv_p1_z. {
-        destruct storage_mixin. destruct protocol_mixin0.
-        setoid_rewrite <- incll. trivial.
-    }
-
-    assert (✓ (interp (p2 ⋅ q ⋅ z) ⋅ b2)) as val_interp2.
-    {
-      destruct storage_mixin. destruct base_ra_mixin0.
-      setoid_rewrite <- interp_eq. trivial.
-    }
-    
-    setoid_rewrite <- f_op; trivial.
-
-    setoid_rewrite interp_eq.
-    setoid_rewrite f_op; trivial.
-    
-    iDestruct "f_op" as "[fi fb]".
-
-    iAssert ((▷ ∃ state0 : P,
-          own γ (● Inved state0) ∗ ⌜pinv state0⌝ ∗ f (interp state0))%I)
-          with "[x fi]"
-          as "inv_to_return".
-    {
-      iModIntro. (* strip later *)
-      iExists (p2 ⋅ q ⋅ z). iFrame "x". iFrame "fi".
-      iPureIntro. trivial.
-    }
-    iDestruct (ownI_close γ _ with "[w m inv_to_return od]") as "[w en]".
-    { iFrame "m". iFrame "inv_to_return". iFrame "w". iFrame "od". }
-    iModIntro. iModIntro. iFrame. iExists p2. iExists b2. iFrame. iPureIntro. trivial.
-  Qed.
-  *)
-  
-  (*
-  Lemma logic_exchange_with_extra_guard_nondeterministic2
-    (p1 q: P) (b1: B) (output_ok: P -> B -> Prop) (γ: gname) (f: B -> iProp Σ) (G: iProp Σ) E
-    (exchng: storage_protocol_exchange_nondeterministic (p1 ⋅ q) b1
-        (λ p2_q b2 , ∃ p2 , p2_q = p2 ⋅ q /\ output_ok p2 b2))
+        (λ p2_q b2 , ∃ p2 , p2_q = p2 ⋅ q ∧ output_ok p2 b2))
     (gname_in_e: γ ∈ E)
-    : maps γ f ∗ □ (G &&{ E }&&> p_own γ q) ⊢
-        G ∗ p_own γ p1 ∗ ▷ f b1 ={ E }=∗ ∃ p2 b2 ,
-            ⌜ output_ok p2 b2 ⌝ ∗ G ∗ p_own γ p2 ∗ ▷ f b2.
-  Proof using B H H0 H1 H2 H3 H4 H5 H6 H7 H8 H9 P equ equb inG0 invGS0 storage_mixin Σ.
-    unfold maps.
-    iIntros "[[%wfm [#ounit #m]] #gu] [g [p f]]".
-    iDestruct (guards_from_inv _ _ E with "m") as "mg". { set_solver. }
-    iDestruct (guards_true E G) as "gt".
-    iDestruct (guards_transitive _ G True%I with "[gt mg]") as "gg".
-    { iFrame "gt". iFrame "mg". }
-    iDestruct (guards_open_two_simultaneously G _ _ E E with "[g gg gu]") as "opened".
-    { set_solver. }
-    { iFrame "g". iSplit. { iFrame "gg". } iFrame "gu". }
-    iMod "opened" as (T) "[t [tinv [town back]]]".
-    
-    iAssert ((◇ own γ (◯ Inved q) ∧ (
-          ◇ (▷ (∃ state : P, own γ (● Inved state) ∗ ⌜pinv state⌝ ∗ f (interp state)) -∗ T)
-          ∗
-          ◇ (∃ state : P, ▷
-                (own γ (● Inved state) ∗ ⌜pinv state⌝ ∗ f (interp state)))
-          ))%I)
-          with "[t tinv town]" as "x".
-    { iSplit. { iMod ("town" with "t") as "town". unfold p_own.
-        iDestruct "town" as "[x y]". iModIntro. iFrame "x". }
-        iDestruct ("tinv" with "t") as "[tinv back]".
-        iFrame "back".
-        iMod "tinv" as "tinv".
-        iMod (bi.later_exist_except_0 with "tinv") as (state0) "tinv".
-        iModIntro.
-        iExists state0.
-        iFrame "tinv".
-    }
-    
-    rewrite <- bi.except_0_sep.
-    rewrite <- bi.except_0_and.
-    iMod "x" as "x".
-    
-    rewrite bi.sep_exist_l.
-    rewrite bi.and_exist_l.
-    iDestruct "x" as (state0) "x".
-    iMod (apply_timeless with "x") as "x".
-    iDestruct (stuff1 with "x") as "%pinvs".
-    unfold p_own.
-    
-    iAssert (own γ (◯ Inved q) ∧ own γ (● Inved state0) ∗ ((▷ (∃ state : P, own γ (● Inved state) ∗ ⌜pinv state⌝ ∗ f (interp state)) -∗ T) ∗ ⌜pinv state0⌝ ∗ ▷ f (interp state0)))%I with "[x]" as "x".
-      { iSplit. { iDestruct "x" as "[x _]". iFrame. }
-          iDestruct "x" as "[_ [x [y z]]]". iFrame. }
-          
-    iDestruct (andsep_to_sepand_ucmra with "x") as "[x y]".
-      { apply auth_frag_disjointness. }
-      
-    iDestruct (own_separates_out γ (◯ Inved q) (own γ (◯ Inved q) ∧ (▷ (∃ state : P, own γ (● Inved state) ∗ ⌜pinv state⌝ ∗ f (interp state)) -∗ T) ∗ ⌜pinv state0⌝ ∗ ▷ f (interp state0)) with "[y]") as "[y z]".
-      { iFrame "y". iIntros "[k _]". iFrame. }
-      
-    iDestruct (own_inved_op p1 q γ with "[p y]") as "own_p_q". { iFrame. }
-    iMod (own_sep_inv_incll_nondet γ (p1 ⋅ q) state0 (λ p2_q r , ∃ p2 b2 , p2_q = p2 ⋅ q /\ output_ok p2 b2
-          /\ pinv ((p2 ⋅ q) ⋅ r)
-          /\ ✓(interp ((p1 ⋅ q) ⋅ r) ⋅ b1)
-          /\ interp ((p1 ⋅ q) ⋅ r) ⋅ b1 ≡ interp ((p2 ⋅ q) ⋅ r) ⋅ b2) with "[own_p_q x]")
-          as (z p2_q) "[%incll [own_p_q x]]".
-      { unfold storage_protocol_exchange_nondeterministic in exchng.
-        intro r. intro j0. have exq := exchng r j0.
-        destruct exq as [p2_q [b2 exq]].
-        destruct exq as [[p2 [eq oo]] [a b]].
-        exists (p2 ⋅ q). split.
-        { exists p2. exists b2. intuition. { rewrite <- eq. apply a. }
-            rewrite <- eq. trivial. }
-        { rewrite <- eq. apply a. }
-      }
-      { apply pinvs. }
-      { iFrame. }
-      
-      destruct incll as [[p2 [b2 [p2_q_eq bigconj]]] incll].
-      rewrite p2_q_eq.
-      iDestruct (own_inved_op_split with "own_p_q") as "[p q]".
-      iDestruct ("z" with "q") as "[_ z]".
-      
-      destruct bigconj as [oo [pix [iix interp_eq]]].
-       
-    destruct wfm as [f_prop [f_unit f_op]]. (* need f Proper for the next step *)
-    
-    assert (f (interp state0)
-          ≡ f(interp (p1 ⋅ q ⋅ z))) as equiv_interp_state.
-    {
-        setoid_rewrite incll. trivial.
-    }
-    
-    iDestruct "z" as "[g [_ fi]]".
-    setoid_rewrite equiv_interp_state.
-    iDestruct (bi.later_sep with "[fi f]") as "f_op". { iFrame "fi". iFrame "f". }
-    
-    unfold storage_protocol_exchange in exchng.
-    assert (pinv (p1 ⋅ q ⋅ z)) as pinv_p1_z. {
-        destruct storage_mixin. destruct protocol_mixin0.
-        setoid_rewrite <- incll. trivial.
-    }
-
-    assert (✓ (interp (p2 ⋅ q ⋅ z) ⋅ b2)) as val_interp2.
-    {
-      destruct storage_mixin. destruct base_ra_mixin0.
-      setoid_rewrite <- interp_eq. trivial.
-    }
-    
-    setoid_rewrite <- f_op; trivial.
-
-    setoid_rewrite interp_eq.
-    setoid_rewrite f_op; trivial.
-    
-    iDestruct "f_op" as "[fi fb]".
-
-    iAssert ((▷ ∃ state0 : P,
-          own γ (● Inved state0) ∗ ⌜pinv state0⌝ ∗ f (interp state0))%I)
-          with "[x fi]"
-          as "inv_to_return".
-    {
-      iModIntro.
-      iExists (p2 ⋅ q ⋅ z). iFrame "x". iFrame "fi".
-      iPureIntro. trivial.
-    }
-    iDestruct ("g" with "inv_to_return") as "g".
-    iMod ("back" with "g") as "g".
-    iModIntro. iFrame. iExists p2. iExists b2. iFrame. iPureIntro. trivial.
-  Qed.
-  *)
-    
-  Lemma logic_exchange_with_extra_guard_nondeterministic_with_later
-    (p1 q: P) (b1: B) (output_ok: P -> B -> Prop) (γ: gname) (f: B -> iProp Σ) (G: iProp Σ) E n
-    (exchng: storage_protocol_exchange_nondeterministic (p1 ⋅ q) b1
-        (λ p2_q b2 , ∃ p2 , p2_q = p2 ⋅ q /\ output_ok p2 b2))
-    (gname_in_e: γ ∈ E)
-    : maps γ f ∗ (G &&{ E ; n }&&> p_own γ q) ⊢
-        G ∗ p_own γ p1 ∗ ▷ f b1 ={ E, ∅ }=∗ ▷^n (|={ ∅, E }=> ∃ p2 b2 ,
-            ⌜ output_ok p2 b2 ⌝ ∗ G ∗ p_own γ p2 ∗ ▷ f b2).
-  Proof using B H H0 H1 H2 H3 H4 H5 H6 H7 H8 H9 P equ equb inG0 invGS0 storage_mixin Σ.
-    unfold maps.
+    : sp_sto γ f ∗ (G &&{ E ; n }&&> sp_own γ q) ⊢
+        G ∗ sp_own γ p1 ∗ ▷ f b1 ={ E, ∅ }=∗ ▷^n (|={ ∅, E }=> ∃ p2 b2 ,
+            ⌜ output_ok p2 b2 ⌝ ∗ G ∗ sp_own γ p2 ∗ ▷ f b2).
+  Proof.
+    unfold sp_sto. rewrite sp_own_eq. unfold sp_own_def.
     iIntros "[[%wfm [#ounit #m]] #gu] [g [p f]]".
     iDestruct (guards_from_inv _ _ E with "m") as "mg". { set_solver. }
     iDestruct (guards_true E G) as "gt".
@@ -1101,13 +776,13 @@ Section StorageLogic.
     iMod "opened" as (T) "[t [tinv [town back]]]".
     
     iAssert ((▷^n (◇ own γ (◯ Inved q) ∧ (
-          ◇ (▷ (∃ state : P, own γ (● Inved state) ∗ ⌜pinv state⌝ ∗ f (interp state)) -∗ T)
+          ◇ (▷ (∃ state_t : (P * B), own γ (● Inved state_t.1) ∗ ⌜sp_rel state_t.1 state_t.2⌝ ∗ f state_t.2) -∗ T)
           ∗
-          ◇ (∃ state : P, ▷
-                (own γ (● Inved state) ∗ ⌜pinv state⌝ ∗ f (interp state)))
+          ◇ (∃ state_t : (P * B), ▷
+                (own γ (● Inved state_t.1) ∗ ⌜sp_rel state_t.1 state_t.2⌝ ∗ f state_t.2))
           )))%I)
           with "[t tinv town]" as "x".
-    { iSplit. { iDestruct ("town" with "t") as "town". iNext. unfold p_own.
+    { iSplit. { iDestruct ("town" with "t") as "town". iNext. unfold sp_own.
         iDestruct "town" as "[x y]". iFrame "x". }
         iDestruct ("tinv" with "t") as "[tinv back]".
         iFrame "back". iNext. iMod "tinv" as "tinv".
@@ -1125,66 +800,58 @@ Section StorageLogic.
     rewrite bi.sep_exist_l.
     rewrite bi.and_exist_l.
     iDestruct "x" as (state0) "x".
-    iMod (apply_timeless with "x") as "x".
-    iDestruct (stuff1 with "x") as "%pinvs".
-    unfold p_own.
+    iMod (apply_timeless_rhs4 with "x") as "x".
+    iDestruct (and_rhs3_entails with "x") as "%pinvs".
+    unfold sp_own.
     
-    iAssert (own γ (◯ Inved q) ∧ own γ (● Inved state0) ∗ ((▷ (∃ state : P, own γ (● Inved state) ∗ ⌜pinv state⌝ ∗ f (interp state)) -∗ T) ∗ ⌜pinv state0⌝ ∗ ▷ f (interp state0)))%I with "[x]" as "x".
+    iAssert (own γ (◯ Inved q) ∧ own γ (● Inved state0.1) ∗ ((▷ (∃ state_t : P * B, own γ (● Inved state_t.1) ∗ ⌜sp_rel state_t.1 state_t.2⌝ ∗ f state_t.2) -∗ T) ∗ ⌜sp_rel state0.1 state0.2⌝ ∗ ▷ f state0.2))%I with "[x]" as "x".
       { iSplit. { iDestruct "x" as "[x _]". iFrame. }
           iDestruct "x" as "[_ [x [y z]]]". iFrame. }
           
     iDestruct (andsep_to_sepand_ucmra with "x") as "[x y]".
       { apply auth_frag_disjointness. }
       
-    iDestruct (own_separates_out γ (◯ Inved q) (own γ (◯ Inved q) ∧ (▷ (∃ state : P, own γ (● Inved state) ∗ ⌜pinv state⌝ ∗ f (interp state)) -∗ T) ∗ ⌜pinv state0⌝ ∗ ▷ f (interp state0)) with "[y]") as "[y z]".
+    iDestruct (own_separates_out γ (◯ Inved q) (own γ (◯ Inved q) ∧ (▷ (∃ state_t : P * B, own γ (● Inved state_t.1) ∗ ⌜sp_rel state_t.1 state_t.2⌝ ∗ f state_t.2) -∗ T) ∗ ⌜sp_rel state0.1 state0.2⌝ ∗ ▷ f state0.2) with "[y]") as "[y z]".
       { iFrame "y". iIntros "[k _]". iFrame. }
       
     iDestruct (own_inved_op p1 q γ with "[p y]") as "own_p_q". { iFrame. }
-    iMod (own_sep_inv_incll_nondet γ (p1 ⋅ q) state0 (λ p2_q r , ∃ p2 b2 , p2_q = p2 ⋅ q /\ output_ok p2 b2
-          /\ pinv ((p2 ⋅ q) ⋅ r)
-          /\ ✓(interp ((p1 ⋅ q) ⋅ r) ⋅ b1)
-          /\ interp ((p1 ⋅ q) ⋅ r) ⋅ b1 ≡ interp ((p2 ⋅ q) ⋅ r) ⋅ b2) with "[own_p_q x]")
+    iMod (own_sep_inv_incll_nondet γ (p1 ⋅ q) state0.1 state0.2 (λ p2_q r , ∃ p2 b2 t2 , p2_q = p2 ⋅ q ∧ output_ok p2 b2
+          ∧ sp_rel ((p2 ⋅ q) ⋅ r) t2
+          ∧ ✓(state0.2 ⋅ b1)
+          ∧ state0.2 ⋅ b1 ≡ t2 ⋅ b2) with "[own_p_q x]")
           as (z p2_q) "[%incll [own_p_q x]]".
       { unfold storage_protocol_exchange_nondeterministic in exchng.
-        intro r. intro j0. have exq := exchng r j0.
-        destruct exq as [p2_q [b2 exq]].
+        intro r. intro j0. have exq := exchng r state0.2 j0.
+        destruct exq as [p2_q [b2 [t2 exq]]].
         destruct exq as [[p2 [eq oo]] [a b]].
-        exists (p2 ⋅ q). split.
-        { exists p2. exists b2. intuition. { rewrite <- eq. apply a. }
-            rewrite <- eq. trivial. }
+        exists (p2 ⋅ q). exists t2. split.
+        { exists p2. exists b2. exists t2. intuition. rewrite <- eq. apply a. }
         { rewrite <- eq. apply a. }
       }
-      { apply pinvs. }
-      { iFrame. }
+    { trivial. }
+    { iFrame. }
       
-      destruct incll as [[p2 [b2 [p2_q_eq bigconj]]] incll].
-      rewrite p2_q_eq.
-      iDestruct (own_inved_op_split with "own_p_q") as "[p q]".
-      iDestruct ("z" with "q") as "[_ z]".
-      
-      destruct bigconj as [oo [pix [iix interp_eq]]].
+    destruct incll as [[p2 [b2 [t2 [p2_q_eq bigconj]]]] incll].
+    rewrite p2_q_eq.
+    iDestruct (own_inved_op_split with "own_p_q") as "[p q]".
+    iDestruct ("z" with "q") as "[_ z]".
+
+    destruct bigconj as [oo [pix [iix interp_eq]]].
        
     destruct wfm as [f_prop [f_unit f_op]]. (* need f Proper for the next step *)
     
-    assert (f (interp state0)
-          ≡ f(interp (p1 ⋅ q ⋅ z))) as equiv_interp_state.
-    {
-        setoid_rewrite incll. trivial.
-    }
-    
     iDestruct "z" as "[g [_ fi]]".
-    setoid_rewrite equiv_interp_state.
     iDestruct (bi.later_sep with "[fi f]") as "f_op". { iFrame "fi". iFrame "f". }
     
     unfold storage_protocol_exchange in exchng.
     assert (pinv (p1 ⋅ q ⋅ z)) as pinv_p1_z. {
-        destruct storage_mixin. destruct protocol_mixin0.
-        setoid_rewrite <- incll. trivial.
+        setoid_rewrite <- incll. exists (state0.2).
+        apply pinvs.
     }
 
-    assert (✓ (interp (p2 ⋅ q ⋅ z) ⋅ b2)) as val_interp2.
+    assert (✓ (t2 ⋅ b2)) as val_interp2.
     {
-      destruct storage_mixin. destruct base_ra_mixin0.
+      destruct (base_ra_mixin _ _ storage_mixin).
       setoid_rewrite <- interp_eq. trivial.
     }
     
@@ -1195,13 +862,13 @@ Section StorageLogic.
     
     iDestruct "f_op" as "[fi fb]".
 
-    iAssert ((▷ ∃ state0 : P,
-          own γ (● Inved state0) ∗ ⌜pinv state0⌝ ∗ f (interp state0))%I)
+    iAssert ((▷ ∃ state0_t : P * B,
+          own γ (● Inved state0_t.1) ∗ ⌜sp_rel state0_t.1 state0_t.2⌝ ∗ f state0_t.2)%I)
           with "[x fi]"
           as "inv_to_return".
     {
       iModIntro.
-      iExists (p2 ⋅ q ⋅ z). iFrame "x". iFrame "fi".
+      iExists (p2 ⋅ q ⋅ z, t2). iFrame "x". iFrame "fi".
       iPureIntro. trivial.
     }
     iDestruct ("g" with "inv_to_return") as "g".
@@ -1209,31 +876,32 @@ Section StorageLogic.
     iModIntro. iFrame. iPureIntro. trivial.
   Qed.
   
-  Lemma logic_exchange_with_extra_guard_nondeterministic
-    (p1 q: P) (b1: B) (output_ok: P -> B -> Prop) (γ: gname) (f: B -> iProp Σ) (G: iProp Σ) E
+  Lemma sp_exchange_with_extra_guard_nondeterministic
+    (p1 q: P) (b1: B) (output_ok: P → B → Prop) (γ: gname) (f: B → iProp Σ) (G: iProp Σ) E
     (exchng: storage_protocol_exchange_nondeterministic (p1 ⋅ q) b1
-        (λ p2_q b2 , ∃ p2 , p2_q = p2 ⋅ q /\ output_ok p2 b2))
+        (λ p2_q b2 , ∃ p2 , p2_q = p2 ⋅ q ∧ output_ok p2 b2))
     (gname_in_e: γ ∈ E)
-    : maps γ f ∗ (G &&{ E }&&> p_own γ q) ⊢
-        G ∗ p_own γ p1 ∗ ▷ f b1 ={ E }=∗ ∃ p2 b2 ,
-            ⌜ output_ok p2 b2 ⌝ ∗ G ∗ p_own γ p2 ∗ ▷ f b2.
-  Proof using B H H0 H1 H10 H2 H3 H4 H5 H6 H7 H8 H9 P equ equb inG0 invGS0 storage_mixin Σ.
+    : sp_sto γ f ∗ (G &&{ E }&&> sp_own γ q) ⊢
+        G ∗ sp_own γ p1 ∗ ▷ f b1 ={ E }=∗ ∃ p2 b2 ,
+            ⌜ output_ok p2 b2 ⌝ ∗ G ∗ sp_own γ p2 ∗ ▷ f b2.
+  Proof.
     iIntros "x y".
-    iDestruct (logic_exchange_with_extra_guard_nondeterministic_with_later p1 q b1 output_ok γ f G E 0 exchng gname_in_e with "x y") as "J".
+    iDestruct (sp_exchange_with_extra_guard_nondeterministic_with_later p1 q b1 output_ok γ f G E 0 exchng gname_in_e with "x y") as "J".
     iMod "J". iMod "J". iModIntro. iFrame.
   Qed.
   
-  Lemma logic_exchange_with_extra_guard
-    (p1 p2 q: P) (b1 b2: B) (γ: gname) (f: B -> iProp Σ) (G: iProp Σ)
+  Lemma sp_exchange_with_extra_guard
+    (p1 p2 q: P) (b1 b2: B) (γ: gname) (f: B → iProp Σ) (G: iProp Σ)
     (exchng: storage_protocol_exchange (p1 ⋅ q) (p2 ⋅ q) b1 b2)
-    : maps γ f ∗ (G &&{ {[ γ ]} }&&> p_own γ q) ⊢
-        G ∗ p_own γ p1 ∗ ▷ f b1 ={ {[ γ ]} }=∗ G ∗ p_own γ p2 ∗ ▷ f b2.
-  Proof using B H H0 H1 H2 H3 H4 H5 H6 H7 H8 H9 P equ equb inG0 invGS0 storage_mixin Σ.
+    : sp_sto γ f ∗ (G &&{ {[ γ ]} }&&> sp_own γ q) ⊢
+        G ∗ sp_own γ p1 ∗ ▷ f b1 ={ {[ γ ]} }=∗ G ∗ sp_own γ p2 ∗ ▷ f b2.
+  Proof.
     iIntros "x y".
-    iDestruct (logic_exchange_with_extra_guard_nondeterministic p1 q b1 (λ p b, p = p2 ∧ b = b2) γ f G {[ γ ]} with "x y") as "J".
+    iDestruct (sp_exchange_with_extra_guard_nondeterministic p1 q b1 (λ p b, p = p2 ∧ b = b2) γ f G {[ γ ]} with "x y") as "J".
     { unfold storage_protocol_exchange_nondeterministic.
       unfold storage_protocol_exchange in exchng.
-      intros q0 pi. exists (p2 ⋅ q). exists b2. have ex := exchng q0 pi.
+      intros q0 t1 pi. exists (p2 ⋅ q). exists b2. have ex := exchng q0 t1 pi.
+      destruct ex as [t2 ex]. exists t2.
       split. { exists p2. split; trivial. split; trivial. }
       apply ex.
     }
@@ -1241,91 +909,43 @@ Section StorageLogic.
     iMod "J" as (p0 b0) "[[%es %es2] L]". iModIntro. subst p0. subst b0. iFrame.
   Qed.
   
-  (*
-  Lemma logic_exchange_nondeterministic
-    (p1: P) (b1: B) (output_ok: P -> B -> Prop) (γ: gname) (f: B -> iProp Σ)
-    (exchng: storage_protocol_exchange_nondeterministic p1 b1 output_ok)
-    : maps γ f ⊢
-        p_own γ p1 ∗ ▷ f b1 ={ {[ γ ]} }=∗
-          ∃ p2 b2 , ⌜ output_ok p2 b2 ⌝ ∗ p_own γ p2 ∗ ▷ f b2.
-  Proof using B H H0 H1 H2 H3 H4 H5 H6 H7 H8 H9 P equ equb inG0 invGS0 storage_mixin Σ.
-    iIntros "maps p_own".
-    iDestruct (logic_exchange_with_extra_guard_nondeterministic p1 ε b1 output_ok γ f True {[ γ ]}) as "J".
-    { unfold storage_protocol_exchange_nondeterministic in *. intros q pi.
-      assert (p1 ⋅ ε ≡ p1) as X. {
-        destruct storage_mixin. destruct protocol_mixin.
-        rewrite ra_comm; trivial.
-      }
-      assert (pinv (p1 ⋅ q)) as Y. {
-        destruct storage_mixin. destruct protocol_mixin.
-          apply inv_proper with (x := (p1 ⋅ ε) ⋅ q); trivial.
-          rewrite ra_comm; trivial.
-          setoid_replace (p1 ⋅ q) with (q ⋅ p1) by (rewrite ra_comm; trivial).
-          have op_proper := (ra_op_proper P protocol_ra_mixin).
-          unfold Proper, "==>", impl in op_proper.
-          have opp := op_proper q (p1 ⋅ ε) p1.
-          apply opp. apply X.
-      }
-      
-      have ex := exchng q Y.
-      destruct ex as [p2 [b2 [oo [pi2 in2]]]].
-      exists (p2 ⋅ ε). exists b2.
-      
-      assert (p2 ⋅ ε ≡ p2) as Z. {
-        destruct storage_mixin. destruct protocol_mixin.
-        rewrite ra_comm; trivial.
-      }
-      assert (pinv (p2 ⋅ ε ⋅ q)) as W. {
-        destruct storage_mixin. destruct protocol_mixin.
-          apply inv_proper with (x := (p2 ⋅ q)); trivial.
-          rewrite ra_comm; trivial.
-          setoid_replace (p2 ⋅ ε ⋅ q) with (q ⋅ (p2 ⋅ ε)) by (rewrite ra_comm; trivial).
-          have op_proper := (ra_op_proper P protocol_ra_mixin).
-          unfold Proper, "==>", impl in op_proper.
-          have opp := op_proper q p2 (p2 ⋅ ε).
-          apply opp. symmetry. apply Z.
-      }
-      intuition.
-      { exists p2. split; trivial. }
-   *)   
-
-    
-  
-  Lemma inved_op (a b : P) :
+  Local Lemma inved_op (a b : P) :
       Inved (a ⋅ b) ≡ Inved a ⋅ Inved b.
-  Proof using H4 H6 H7 P equ. trivial. Qed.
+  Proof using equ_p. trivial. Qed.
 
   (* SP-Sep *)
 
-  Lemma p_own_op a b γ :
-      p_own γ (a ⋅ b) ⊣⊢ p_own γ a ∗ p_own γ b.
+  Lemma sp_own_op a b γ :
+      sp_own γ (a ⋅ b) ⊣⊢ sp_own γ a ∗ sp_own γ b.
   Proof.
-    unfold p_own.
+    rewrite sp_own_eq. unfold sp_own_def.
     setoid_rewrite inved_op.
     rewrite auth_frag_op.
     apply own_op.
   Qed.
   
+  (* TODO
+  Lemma sp_own_and x y γ :
+      sp_own γ x ∧ sp_own γ y ⊢ ∃ z , ⌜ x ≼ z ∧ y ≼ z ⌝ ∗ sp_own γ z.
+  Proof.
+    iIntros "H". unfold sp_own. iDestruct (and_own_discrete_ucmra with "H") as (z) "[J %t]".
+    destruct t as [Hxz Hyz]. destruct z as [|p].
+  Qed.
+  *)
+  
   Lemma op_unit (p: P) : p ⋅ ε ≡ p.
-  Proof using B H H0 H1 H2 H3 H4 H5 H6 H7 H8 H9 P equ inG0 storage_mixin Σ.
-    destruct storage_mixin.
-    destruct protocol_mixin.
-    destruct protocol_ra_mixin.
-    setoid_rewrite (@comm P).
-    - apply protocol_unit_left_id.
-    - trivial.
+  Proof using storage_mixin.
+    rewrite (ra_comm _ (protocol_ra_mixin _ _ storage_mixin)).
+    apply (protocol_unit_left_id _ _ storage_mixin).
   Qed.
   
   Lemma op_unit_base (b: B) : b ⋅ ε ≡ b.
-  Proof using B H H0 H1 H2 H3 H4 H5 H6 H7 H8 H9 P equ equb inG0 storage_mixin Σ.
-    destruct storage_mixin.
-    destruct base_ra_mixin0.
-    setoid_rewrite (@comm B).
-    - apply base_unit_left_id0.
-    - trivial.
+  Proof using storage_mixin.
+    rewrite (ra_comm _ (base_ra_mixin _ _ storage_mixin)).
+    apply (base_unit_left_id _ _ storage_mixin).
   Qed.
   
-  Lemma auth_inved_conjure_unit γ (state: P)
+  Local Lemma auth_inved_conjure_unit γ (state: P)
       : own γ (● Inved state) ==∗ own γ (● Inved state) ∗ own γ (◯ Inved ε).
   Proof.
       apply auth_conjure_frag.
@@ -1333,28 +953,34 @@ Section StorageLogic.
       setoid_rewrite op_unit.
       trivial.
   Qed.
+   
+  Local Lemma valid_inved_of_pinv (p: P)
+    : pinv p → ✓ (Inved p). 
+  Proof using storage_mixin.
+    intro pi. unfold "✓", inved_protocol_valid. exists ε. setoid_rewrite op_unit.
+    trivial.
+  Qed.
 
   (* SP-Unit *)
   
-  Lemma p_own_unit γ f
-      : maps γ f ⊢ p_own γ ε.
-  Proof using B H H0 H1 H2 H3 H4 H5 H6 H7 H8 H9 P equ equb inG0 invGS0 storage_mixin Σ.
-    unfold maps.
+  Lemma sp_own_unit γ f
+      : sp_sto γ f ⊢ sp_own γ ε.
+  Proof.
+    unfold sp_sto. rewrite sp_own_eq. unfold sp_own_def.
     iIntros "[%wfm [#ounit #m]]".
-    unfold p_own.
     iFrame "ounit".
   Qed.
 
   (* SP-Deposit *)
     
-  Lemma logic_deposit
-      (p1 p2: P) (b1: B) (γ: gname) (f: B -> iProp Σ)
+  Lemma sp_deposit
+      (p1 p2: P) (b1: B) (γ: gname) (f: B → iProp Σ)
       (exchng: storage_protocol_deposit p1 p2 b1)
-      : maps γ f ⊢
-          p_own γ p1 ∗ ▷ f b1 ={ {[ γ ]} }=∗ p_own γ p2.
-   Proof using B H H0 H1 H2 H3 H4 H5 H6 H7 H8 H9 P equ equb inG0 invGS0 storage_mixin Σ.
+      : sp_sto γ f ⊢
+          sp_own γ p1 ∗ ▷ f b1 ={ {[ γ ]} }=∗ sp_own γ p2.
+  Proof.
     iIntros "#m pb".
-    iMod (logic_exchange p1 p2 b1 (ε: B) γ f with "m pb") as "[pb u]".
+    iMod (sp_exchange p1 p2 b1 (ε: B) γ f with "m pb") as "[pb u]".
     {
       unfold storage_protocol_exchange.
       unfold storage_protocol_deposit in exchng.
@@ -1363,107 +989,87 @@ Section StorageLogic.
       trivial.
     }
     iModIntro. iFrame "pb".
-   Qed.
+  Qed.
    
   Instance valid_proper_base : Proper ((≡) ==> impl) (@valid B _).
-  Proof using B H H0 H1 H2 H3 H4 H5 H6 H7 H8 H9 P equ inG0 storage_mixin Σ.
-    destruct storage_mixin.
-    destruct base_ra_mixin0.
-    apply ra_validN_proper.
+  Proof using storage_mixin.
+    apply (ra_validN_proper _ (base_ra_mixin _ _ storage_mixin)).
   Qed.
   
-  Instance pinv_proper : Proper ((≡) ==> impl) (@pinv P _).
-  Proof using B H H0 H1 H2 H3 H4 H5 H6 H7 H8 H9 P equ inG0 storage_mixin Σ.
-    destruct storage_mixin.
-    destruct protocol_mixin0.
-    apply inv_proper.
-  Qed.
-  
-  Lemma valid_interp (p: P)
-      : pinv p -> ✓ (interp p).
-  Proof using B H H0 H1 H2 H3 H4 H5 H6 H7 H8 H9 P equ inG0 storage_mixin Σ.
-    destruct storage_mixin.
-    apply interp_val0.
-  Qed.
-
   (* SP-Withdraw *)
    
-  Lemma logic_withdraw
-      (p1 p2: P) (b2: B) (γ: gname) (f: B -> iProp Σ)
+  Lemma sp_withdraw
+      (p1 p2: P) (b2: B) (γ: gname) (f: B → iProp Σ)
       (exchng: storage_protocol_withdraw p1 p2 b2)
-      : maps γ f ⊢
-          p_own γ p1 ={ {[ γ ]} }=∗ p_own γ p2 ∗ ▷ f b2.
-  Proof using B H H0 H1 H2 H3 H4 H5 H6 H7 H8 H9 P equ equb inG0 invGS0 storage_mixin Σ.
+      : sp_sto γ f ⊢
+          sp_own γ p1 ={ {[ γ ]} }=∗ sp_own γ p2 ∗ ▷ f b2.
+  Proof.
     iIntros "#m pb".
     iAssert (▷ f ε)%I as "u".
     {
       iModIntro. 
-      unfold maps.
+      unfold sp_sto.
       iDestruct "m" as "[%wf #m]".
       unfold wf_prop_map in wf.
       destruct wf as [wf_prop [wf_unit _]].
       setoid_rewrite wf_unit. done.
     }
-    iMod (logic_exchange p1 p2 (ε: B) b2 γ f with "m [pb u]") as "[pb fb2]".
+    iMod (sp_exchange p1 p2 (ε: B) b2 γ f with "m [pb u]") as "[pb fb2]".
     {
       unfold storage_protocol_exchange.
       unfold storage_protocol_withdraw in exchng.
-      intros q pi1. have t := exchng q pi1. intuition.
+      intros q t1 pi1. have j := exchng q t1 pi1. destruct j as [t2 j].
+      exists t2. intuition.
       - setoid_rewrite op_unit_base.
-        apply valid_interp. trivial.
+        destruct storage_mixin. apply (interp_val _ _ storage_mixin (p1 ⋅ q)). trivial.
       - setoid_rewrite op_unit_base. trivial.
     }
     { iFrame "pb". iFrame "u". }
     iModIntro. iFrame.
-   Qed.
+  Qed.
 
   (* SP-Update *)
    
-  Lemma logic_update
-      (p1 p2: P) (γ: gname) (f: B -> iProp Σ)
+  (* TODO It should be possible to do the update at mask ∅, but this requires changing
+     the underlying auth resource slightly. *)
+  Lemma sp_update
+      (p1 p2: P) (γ: gname) (f: B → iProp Σ)
       (exchng: storage_protocol_update p1 p2)
-      : maps γ f ⊢
-          p_own γ p1 ={ {[ γ ]} }=∗ p_own γ p2.
-  Proof using B H H0 H1 H2 H3 H4 H5 H6 H7 H8 H9 P equ equb inG0 invGS0 storage_mixin Σ.
+      : sp_sto γ f ⊢
+          sp_own γ p1 ={ {[ γ ]} }=∗ sp_own γ p2.
+  Proof.
     iIntros "#m pb".
-    iDestruct (logic_withdraw p1 p2 ε γ f with "m pb") as "pb".
+    iDestruct (sp_withdraw p1 p2 ε γ f with "m pb") as "pb".
     {
       unfold storage_protocol_withdraw.
       unfold storage_protocol_update in exchng.
-      intros q pi.
-      have exch := exchng q.
+      intros q t1 pi.
+      have exch := exchng q t1.
       intuition.
-      setoid_rewrite op_unit_base.
-      trivial.
+      setoid_rewrite op_unit_base. exists t1. split; trivial.
     }
     iMod "pb".
     iModIntro.
     iDestruct "pb" as "[pb _]".
     iFrame.
   Qed.
-  
-  Lemma valid_inved_of_pinv (p: P)
-    : pinv p -> ✓ (Inved p). 
-  Proof using B H H0 H1 H2 H3 H4 H5 H6 H7 H8 H9 P equ inG0 storage_mixin Σ.
-    intro pi. unfold "✓", inved_protocol_valid. exists ε. setoid_rewrite op_unit.
-    trivial.
-  Qed.
-
+ 
   (* SP-Alloc *)
   
-  Lemma logic_init_ns (p: P) (f: B -> iProp Σ) E (N: namespace)
-      (pi: pinv p) (wf: wf_prop_map f)
-  : ⊢ f (interp p) ={E}=∗ ∃ γ , ⌜ γ ∈ (↑ N : coPset) ⌝ ∗ maps γ f ∗ p_own γ p.
-  Proof using B H H0 H1 H2 H3 H4 H5 H6 H7 H8 H9 P equ equb inG0 invGS0 storage_mixin Σ.
+  Lemma sp_alloc_ns (p: P) (b: B) (f: B → iProp Σ) E (N: namespace)
+      (pi: sp_rel p b) (wf: wf_prop_map f)
+  : ⊢ f b ={E}=∗ ∃ γ , ⌜ γ ∈ (↑ N : coPset) ⌝ ∗ sp_sto γ f ∗ sp_own γ p.
+  Proof.
     iIntros "f_init".
+    rewrite sp_own_eq. unfold sp_own_def.
     rewrite fancy_updates.uPred_fupd_unseal. unfold fancy_updates.uPred_fupd_def.
     iIntros "[w oe]".
     iMod (ownI_alloc_and_simultaneous_own_alloc_ns
       (λ γ , 
-        (∃ (state: P) ,
-          own γ (● (Inved state))
-          ∗ ⌜ pinv state ⌝
-          ∗ (f (interp state)))%I
+        (∃ (state_t: P * B) ,
+          own γ (● (Inved state_t.1))
+          ∗ ⌜ sp_rel state_t.1 state_t.2 ⌝
+          ∗ (f state_t.2))%I
       )
       (● (Inved p) ⋅ (◯ (Inved ε) ⋅ ◯ (Inved p)))
       (↑ N)
@@ -1473,39 +1079,39 @@ Section StorageLogic.
       rewrite <- auth_frag_op.
       rewrite auth_both_valid_discrete. split; trivial.
       - replace (Inved ε ⋅ Inved p) with (Inved (ε ⋅ p)) by trivial.
-        destruct storage_mixin. destruct protocol_mixin0. rewrite protocol_unit_left_id.
+        rewrite (protocol_unit_left_id _ _ storage_mixin).
         trivial.
-      - apply valid_inved_of_pinv. trivial.
+      - apply valid_inved_of_pinv. exists b. apply pi.
     }
     
     iDestruct "w" as (γ) "[%in_ns [w [oinv [auth [u frag]]]]]".
     
     iDestruct ("w" with "[auth f_init]") as "w".
     {
-      iModIntro. iExists p. iFrame. iPureIntro. trivial.
+      iModIntro. iExists (p, b). iFrame. iPureIntro. trivial.
     }
     
     iModIntro. iModIntro.
     iFrame "w". iFrame "oe".
     iExists γ.
-    unfold p_own. iFrame "frag".
-    unfold maps.
+    unfold sp_own. iFrame "frag".
+    unfold sp_sto.
     iFrame "oinv". iFrame.
     iPureIntro. split; trivial.
   Qed.
   
-  Lemma logic_init (p: P) (f: B -> iProp Σ) E
-      (pi: pinv p) (wf: wf_prop_map f)
-  : ⊢ f (interp p) ={E}=∗ ∃ γ , maps γ f ∗ p_own γ p.
-  Proof using B H H0 H1 H2 H3 H4 H5 H6 H7 H8 H9 P equ equb inG0 invGS0 storage_mixin Σ.
+  Lemma sp_alloc (p: P) (b: B) (f: B → iProp Σ) E
+      (pi: sp_rel p b) (wf: wf_prop_map f)
+  : ⊢ f b ={E}=∗ ∃ γ , sp_sto γ f ∗ sp_own γ p.
+  Proof.
     iIntros "f_init".
-    iMod (logic_init_ns p f E nroot with "f_init") as (γ) "[_ t]"; trivial.
+    iMod (sp_alloc_ns p b f E nroot with "f_init") as (γ) "[_ t]"; trivial.
     iModIntro. iExists γ. iFrame.
   Qed.
   
   Lemma fupd_singleton_mask_frame (γ: gname) (X Y Z : iProp Σ) E
     (premise: X ⊢ Y ={ {[ γ ]} }=∗ Z) (is_in: γ ∈ E) : X ⊢ Y ={ E }=∗ Z.
-  Proof using B H equb invGS0 Σ.
+  Proof.
     iIntros "x y".
     iDestruct (premise with "x y") as "p".
     iDestruct (fupd_mask_frame_r _ _ (E ∖ {[γ]}) with "p") as "p".
@@ -1518,66 +1124,94 @@ Section StorageLogic.
     trivial.
   Qed.
     
-  Lemma logic_exchange'
-    (p1 p2: P) (b1 b2: B) (γ: gname) (f: B -> iProp Σ) E
+  Lemma sp_exchange'
+    (p1 p2: P) (b1 b2: B) (γ: gname) (f: B → iProp Σ) E
     (exchng: storage_protocol_exchange p1 p2 b1 b2)
     (gname_in_e: γ ∈ E)
-    : maps γ f ⊢
-        p_own γ p1 ∗ ▷ f b1 ={ E }=∗ p_own γ p2 ∗ ▷ f b2.
-  Proof using B H H0 H1 H2 H3 H4 H5 H6 H7 H8 H9 P equ equb inG0 invGS0 storage_mixin Σ.
+    : sp_sto γ f ⊢
+        sp_own γ p1 ∗ ▷ f b1 ={ E }=∗ sp_own γ p2 ∗ ▷ f b2.
+  Proof.
     apply (fupd_singleton_mask_frame γ); trivial.
-    apply logic_exchange; trivial.
+    apply sp_exchange; trivial.
   Qed.
    
-  Lemma logic_deposit'
-      (p1 p2: P) (b1: B) (γ: gname) (f: B -> iProp Σ) E
+  Lemma sp_deposit'
+      (p1 p2: P) (b1: B) (γ: gname) (f: B → iProp Σ) E
       (exchng: storage_protocol_deposit p1 p2 b1)
       (gname_in_e: γ ∈ E)
-      : maps γ f ⊢
-          p_own γ p1 ∗ ▷ f b1 ={ E }=∗ p_own γ p2.
-   Proof using B H H0 H1 H2 H3 H4 H5 H6 H7 H8 H9 P equ equb inG0 invGS0 storage_mixin Σ.
+      : sp_sto γ f ⊢
+          sp_own γ p1 ∗ ▷ f b1 ={ E }=∗ sp_own γ p2.
+  Proof.
     apply (fupd_singleton_mask_frame γ); trivial.
-    apply logic_deposit; trivial.
-   Qed.
-
-  Lemma logic_withdraw'
-      (p1 p2: P) (b2: B) (γ: gname) (f: B -> iProp Σ) E
-      (exchng: storage_protocol_withdraw p1 p2 b2)
-      (gname_in_e: γ ∈ E)
-      : maps γ f ⊢
-          p_own γ p1 ={ E }=∗ p_own γ p2 ∗ ▷ f b2.
-  Proof using B H H0 H1 H2 H3 H4 H5 H6 H7 H8 H9 P equ equb inG0 invGS0 storage_mixin Σ.
-    apply (fupd_singleton_mask_frame γ); trivial.
-    apply logic_withdraw; trivial.
+    apply sp_deposit; trivial.
   Qed.
 
-  Lemma logic_update'
-      (p1 p2: P) (γ: gname) (f: B -> iProp Σ) E
+  Lemma sp_withdraw'
+      (p1 p2: P) (b2: B) (γ: gname) (f: B → iProp Σ) E
+      (exchng: storage_protocol_withdraw p1 p2 b2)
+      (gname_in_e: γ ∈ E)
+      : sp_sto γ f ⊢
+          sp_own γ p1 ={ E }=∗ sp_own γ p2 ∗ ▷ f b2.
+  Proof.
+    apply (fupd_singleton_mask_frame γ); trivial.
+    apply sp_withdraw; trivial.
+  Qed.
+
+  Lemma sp_update'
+      (p1 p2: P) (γ: gname) (f: B → iProp Σ) E
       (exchng: storage_protocol_update p1 p2)
       (gname_in_e: γ ∈ E)
-      : maps γ f ⊢
-          p_own γ p1 ={ E }=∗ p_own γ p2.
-  Proof using B H H0 H1 H2 H3 H4 H5 H6 H7 H8 H9 P equ equb inG0 invGS0 storage_mixin Σ.
+      : sp_sto γ f ⊢
+          sp_own γ p1 ={ E }=∗ sp_own γ p2.
+  Proof.
     apply (fupd_singleton_mask_frame γ); trivial.
-    apply logic_update; trivial.
+    apply sp_update; trivial.
   Qed.
   
   (* SP-PointProp *)
   
-  Lemma point_prop_p_own (γ: gname) (p: P) : point_prop (p_own γ p).
+  Lemma point_prop_p_own (γ: gname) (p: P) : point_prop (sp_own γ p).
   Proof.
-    unfold p_own. apply point_prop_own.
+    rewrite sp_own_eq. unfold sp_own_def. apply point_prop_own.
   Qed.
   
   (* SP-Valid *)
   
-  Lemma p_own_valid (γ: gname) (p: P)
-      : (p_own γ p) ⊢ ⌜ ∃ q , pinv (p ⋅ q) ⌝.
+  Lemma sp_own_valid (γ: gname) (p: P)
+      : (sp_own γ p) ⊢ ⌜ ∃ q b , sp_rel (p ⋅ q) b ⌝.
   Proof.
+    rewrite sp_own_eq. unfold sp_own_def.
     iIntros "x".  iDestruct (own_valid with "x") as "%x". iPureIntro.
     generalize x. clear x.
     rewrite auth_frag_valid.
     trivial.
   Qed.
- 
+   
+  Global Instance proper_sp_own γ : Proper ((≡) ==> (⊣⊢)) (sp_own γ).
+  Proof. rewrite sp_own_eq. unfold sp_own_def. intros x y Heq.
+      setoid_rewrite Heq. trivial. Qed.
+  
+  Global Instance timeless_sp_own γ a : Timeless (sp_own γ a).
+  Proof. rewrite sp_own_eq. apply _. Qed.
+  
+  Lemma sp_own_mono γ a1 a2 : a2 ≼ a1 → sp_own γ a1 ⊢ sp_own γ a2.
+  Proof.
+    intros [t Heq]. setoid_rewrite Heq. setoid_rewrite sp_own_op.
+    iIntros "[Ha Hb]". iFrame.
+  Qed.
+  
+  Global Instance mono_sp_own' γ : Proper (flip (≼) ==> (⊢)) (sp_own γ).
+  Proof.
+    intros a1 a2. apply sp_own_mono.
+  Qed.
+  
+  Lemma sp_own_core_persistent γ a : (pcore a ≡ Some a) → Persistent (sp_own γ a).
+  Proof.
+    rewrite sp_own_eq. unfold sp_own_def.
+    intros Ha. apply own_core_persistent. apply auth_frag_core_id.
+    unfold CoreId, pcore, cmra_pcore, cmra_pcore. simpl. unfold inved_protocolUR, ucmra_pcore.
+    unfold inved_protocol_pcore.  destruct (pcore a) as [t|].
+    - inversion Ha as [x y Hb Hc Hd|]. setoid_rewrite Hb. trivial.
+    - inversion Ha.
+  Qed.
 End StorageLogic.
